increments for intersection types

double_anno_inter/coq/syntax.v
@@ -1,25 +1,50 @@
 
 (*
-This is the main syntax file as of January 08, 2021
-typing.v is the main typing file
+Update started on March 09, 2021
+
+This is the main syntax file for disjoint union types
+with intersection types.
 *)
 
 (*
-This file contains the updates suggested by Bruno.
-Mutual dependency of algorithmic bottom-like and
-algorithmic disjointness.
+This file contains the updates suggested by Bruno with Bool and String primitive type.
+
+Redundant subtyping rule from bottom type removed in this version.
+
+Subtying algorithm with Coq definition added in this version
+
+A *a B = findsubtypes A `inter` findsubtypes B == []
+
+FindSubtypes B = []
+-------------------
+     B <: A
+
+Transitivity Proved
+
+Bool and String primitive type
+
+******************************************************************
+Redundant subtyping rule for bottom type removed in this version.
+******************************************************************
+
 *)
 
 Require Import TLC.LibLN.
 Require Import Program.Equality.
+Require Import Coq.Lists.ListSet.
+From Coq Require Export Lists.List.
+Export ListNotations.
+Require Import Coq.Strings.String.
 
 (* Require Import LibTactics. *)
 (*Implicit Types x : var.*)
 (** syntax *)
 
 Inductive typ : Set :=  (*r type *)
- | typ_top : typ
+ | t_top : typ
  | t_int : typ
+ | t_bool : typ
+ | t_str : typ
  | t_bot : typ
  | t_arrow : typ -> typ -> typ
  | t_union : typ -> typ -> typ
@@ -29,6 +54,8 @@ Inductive exp : Set :=  (*r expression *)
  | e_var_b  : nat -> exp
  | e_var_f  : var -> exp
  | e_lit    : nat -> exp
+ | e_bool   : bool -> exp
+ | e_str    : string -> exp
  | e_ann    : exp -> typ -> exp
  | e_abs    : exp -> exp
  | e_app    : exp -> exp -> exp
@@ -49,7 +76,6 @@ Notation "x ~: T" := (x ~ T)
 
 (** Environment is an associative list of bindings. *)
 
-
  Definition env := LibEnv.env typ.
 
 Inductive okt : env -> Prop :=
@@ -57,7 +83,6 @@ Inductive okt : env -> Prop :=
      okt empty
 | okt_typ : forall E x T,
      okt E-> x # E -> okt (E & x ~: T).
-
 
 (* EXPERIMENTAL *)
 (** auxiliary functions on the new list types *)
@@ -70,6 +95,8 @@ Fixpoint open_exp_wrt_exp_rec (k:nat) (e_5:exp) (e__6:exp) {struct e__6}: exp :=
   | (e_var_b nat) => If (k = nat) then e_5 else (e_var_b nat)
   | (e_var_f x) => e_var_f x
   | (e_lit i5) => e_lit i5
+  | (e_bool b)=> e_bool b
+  | (e_str s)=> e_str s
   | (e_ann e A) => e_ann (open_exp_wrt_exp_rec k e_5 e) A
   | (e_abs e) => e_abs (open_exp_wrt_exp_rec (S k) e_5 e)
   | (e_app e1 e2) => e_app (open_exp_wrt_exp_rec k e_5 e1) (open_exp_wrt_exp_rec k e_5 e2)
@@ -92,6 +119,10 @@ Inductive lc_exp : exp -> Prop :=    (* defn lc_exp *)
      (lc_exp (e_var_f x))
  | lc_e_lit : forall i5,
      (lc_exp (e_lit i5))
+ | lc_e_bool : forall b,
+     (lc_exp (e_bool b))
+ | lc_e_str : forall s,
+     (lc_exp (e_str s))
  | lc_e_ann : forall (e:exp) (A:typ),
      (lc_exp e) ->
      (lc_exp (e_ann e A))
@@ -113,6 +144,8 @@ Fixpoint fv_exp (e_5:exp) : vars :=
   | (e_var_b nat) => \{}
   | (e_var_f x) => \{x}
   | (e_lit i5) => \{}
+  | (e_bool b) => \{}
+  | (e_str s) => \{}
   | (e_ann e A) => (fv_exp e)
   | (e_abs e) => (fv_exp e)
   | (e_app e1 e2) => (fv_exp e1) \u (fv_exp e2)
@@ -125,12 +158,13 @@ Fixpoint subst_exp (e_5:exp) (x5:var) (e__6:exp) {struct e__6} : exp :=
   | (e_var_b nat) => e_var_b nat
   | (e_var_f x) => (If x = x5 then e_5 else (e_var_f x))
   | (e_lit i5) => e_lit i5
+  | (e_bool b) => e_bool b
+  | (e_str s) => e_str s
   | (e_ann e A) => e_ann (subst_exp e_5 x5 e) A
   | (e_abs e) => e_abs (subst_exp e_5 x5 e)
   | (e_app e1 e2) => e_app (subst_exp e_5 x5 e1) (subst_exp e_5 x5 e2)
   | (e_typeof e A e1 B e2) => e_typeof (subst_exp e_5 x5 e) A (subst_exp e_5 x5 e1) B (subst_exp e_5 x5 e2)
 end.
-
 
 (** definitions *)
 
@@ -138,21 +172,13 @@ end.
 Inductive pexpr : exp -> Prop :=    (* defn pexpr *)
  | pexpr_int : forall i5,
      pexpr (e_lit i5)
+ | pexpr_bool : forall b,
+     pexpr (e_bool b)
+ | pexpr_str : forall s,
+     pexpr (e_str s)
  | pexpr_abs : forall (e:exp) (A B:typ),
      lc_exp (e_abs e) ->
      pexpr (e_ann  ( (e_abs e) )  (t_arrow A B)).
-
-(* defns RExpr *)
-Inductive rexpr : exp -> Prop :=    (* defn rexpr *)
- | rexpr_app : forall (e1 e2:exp),
-     lc_exp e1 ->
-     lc_exp e2 ->
-     rexpr  ( (e_app e1 e2) )
- | rexpr_typeof : forall (e:exp) (A:typ) (e1:exp) (B:typ) (e2:exp),
-     lc_exp e ->
-     lc_exp e1 ->
-     lc_exp e2 ->
-     rexpr (e_typeof e A e1 B e2).
 
 (* defns Value *)
 Inductive value : exp -> Prop :=    (* defn value *)
@@ -160,35 +186,52 @@ Inductive value : exp -> Prop :=    (* defn value *)
      pexpr p ->
      value (e_ann p A).
 
-(* defns UExpr *)
-Inductive uexpr : exp -> Prop :=    (* defn uexpr *)
- | uexpr_rexpr : forall (r:exp),
-     rexpr r ->
-     uexpr r
- | uexpr_pexpr : forall (p:exp),
-     pexpr p ->
-     uexpr p
- | uexpr_anno : forall (u:exp) (A:typ),
-     uexpr u ->
-     uexpr (e_ann u A).
-
 (* defns FindType *)
 Inductive findtype : exp -> typ -> Prop :=    (* defn findtype *)
  | findtype_int : forall i5,
      findtype (e_lit i5) t_int
+ | findtype_bool : forall b,
+     findtype (e_bool b) t_bool
+ | findtype_str : forall s,
+     findtype (e_str s) t_str
  | findtype_arrow : forall (e:exp) (A B:typ),
      lc_exp (e_abs e) ->
      findtype  ( (e_ann  ( (e_abs e) )  (t_arrow A B)) )   (t_arrow A B).
 
+(****************************************)
+(**********  FindSubtypes    ************)
+(****************************************)
+
+Lemma eq_dec : forall x y:typ, {x = y} + {x <> y}.
+Proof.
+ decide equality; auto.
+Defined.
+
+Notation "l1 `union` l2" := (set_union eq_dec l1 l2) (at level 80).
+Notation "l1 `inter` l2" := (set_inter eq_dec l1 l2) (at level 80).
+
+Fixpoint FindSubtypes (A: typ) :=
+    match A with
+    | t_top         => [t_int; t_bool; t_str; t_arrow t_top t_bot; t_top]
+    | t_bot         => []
+    | t_int         => [t_int]
+    | t_bool        => [t_bool]
+    | t_str         => [t_str]
+    | t_arrow A1 B1 => [t_arrow t_top t_bot]
+    | t_union A1 B1 => (FindSubtypes A1) `union` (FindSubtypes B1)
+    | t_and A1 B1   => (FindSubtypes A1) `inter` (FindSubtypes B1)
+    end.
 
 (* defns Subtyping *)
 Reserved Notation "A <: B" (at level 80).
 Inductive subtyping : typ -> typ -> Prop :=    (* defn subtyping *)
- | s_top : forall A, A <: typ_top
- | s_btm : forall (A:typ),
-     t_bot <: A
+ | s_top : forall A, A <: t_top
  | s_int :
-     subtyping t_int t_int
+     t_int <: t_int
+ | s_bool :
+     t_bool <: t_bool
+ | s_str :
+     t_str <: t_str
  | s_arrow : forall (A1 A2 B1 B2:typ),
      B1 <: A1 ->
      A2 <: B2 ->
@@ -213,13 +256,87 @@ Inductive subtyping : typ -> typ -> Prop :=    (* defn subtyping *)
  | s_andc : forall A1 A2 A,
      A2 <: A ->
      (t_and A1 A2) <: A
+ | s_disj : forall A B,
+     FindSubtypes A = [] ->
+     A <: B
 where "A <: B" := (subtyping A B) : env_scope.
 
-Hint Constructors pexpr rexpr value uexpr findtype subtyping lc_exp ok okt.
+Hint Constructors pexpr value findtype subtyping lc_exp ok okt.
+
+(*************************)
+(***** Ordinary Types ****)
+(*************************)
+
+Inductive Ord : typ -> Prop :=
+| o_top   : Ord t_top
+| o_int   : Ord t_int
+| o_bool  : Ord t_bool
+| o_str   : Ord t_str
+| o_arrow : forall t1 t2, Ord (t_arrow t1 t2).
+(*| o_union : forall t1 t2, Ord t1 -> Ord t2 -> Ord (t_union t1 t2).*)
+
+Hint Constructors Ord : core.
 
 (**********************************)
 (*****  Subtyping Properties  *****)
 (**********************************)
+
+Lemma list_empty_decide : forall l : list typ, (l = []) \/ (l <> []).
+Proof.
+  intros. induction l. auto.
+  destruct IHl. right. 
+  unfold not. intros. inversion H0.
+  unfold not in *.
+  right. intros.
+  inversion H0.
+Defined.
+
+Lemma elem_append_in_list : forall (a : typ) (l : list typ), set_In a (a :: l).
+Proof.
+  intros. simpl. auto.
+Defined.
+
+Lemma elem_append_in_union1 : forall (a1 a2 : typ) (l1 l2 : list typ), 
+set_In a1 (a1 :: l1 `union` a2 :: l2).
+Proof.
+  intros.
+  lets: elem_append_in_list a1 l1.
+  apply set_union_intro1. auto.
+Defined.
+
+Lemma elem_append_in_union2 : forall (a1 : typ) (l1 : list typ), 
+set_In a1 ([] `union` a1 :: l1).
+Proof.
+  intros.
+  lets: elem_append_in_list a1 l1.
+  apply set_union_intro2. auto.
+Defined.
+
+Lemma union_findsubtypes_empty_elim : forall l1 A B l2 l3, 
+l1 = FindSubtypes (t_union A B) /\ 
+l2 = FindSubtypes A /\ l3 = FindSubtypes B ->
+l1 = [] -> l2 = [] /\ l3 = [].
+Proof.
+    intros.
+    destructs H.
+    simpl in H.
+    destruct l2.
+    destruct l3.
+    auto.
+    rewrite <- H2 in H.
+    rewrite H0 in H.
+    rewrite <- H1 in H.
+    lets: elem_append_in_union2 t l3.
+    rewrite <- H in H3.
+    inverts H3.
+    rewrite H0 in H.
+    rewrite <- H1 in H.
+    destruct (FindSubtypes B).
+    simpl in H. inverts H.
+    lets: elem_append_in_union1 t t0 l2 l.
+    rewrite <- H in H3.
+    inverts H3.
+Defined.
 
 Lemma sub_or : forall A B C, (t_union A B) <: C -> A <: C /\ B <: C.
 Proof.
@@ -231,6 +348,9 @@ forwards* : IHsubtyping.
 specialize (IHsubtyping1 A B).
 specialize (IHsubtyping2 A B).
 forwards*: IHsubtyping1.
+lets: union_findsubtypes_empty_elim  (FindSubtypes (t_union A B)) A B.
+lets: H0 (FindSubtypes A) (FindSubtypes B).
+forwards*: H1.
 Defined.
 
 Lemma sub_and : forall A B C, A <: (t_and B C) -> A <: B /\ A <: C.
@@ -245,12 +365,466 @@ specialize (IHsubtyping B C).
 forwards*: IHsubtyping.
 Defined.
 
+Lemma arrow_in_top_bot : forall A B C, 
+set_In (t_arrow A B) (FindSubtypes C) ->
+t_arrow A B = t_arrow t_top t_bot.
+Proof.
+  intros. inductions C; try solve [simpl in H; destruct H; inversion H].
+ - simpl in H. destruct H. inversion H.
+   destruct H. inversion H.
+   destruct H. inversion H.
+   destruct H. inversion H. auto.
+   destruct H. inversion H.
+   inversion H.
+ - simpl in H. destruct H. inversion H. auto. inversion H.
+ - simpl in H.
+   apply set_union_elim in H. destruct H.
+   apply IHC1; auto.
+   apply IHC2; auto.
+ - simpl in H.
+   apply set_inter_elim1 in H.
+   apply IHC1; auto.
+Defined.
+
+Lemma ord_in_findsubtypes2 : forall A B,
+Ord A -> A <: B -> set_In A (FindSubtypes B) \/ 
+(exists t1 t2, A = t_arrow t1 t2 /\ set_In (t_arrow t_top t_bot) (FindSubtypes B)).
+Proof.
+  induction 1; intros.
+  - induction B; simpl; auto.
+   + left. right. right. right. auto.
+   + inversion H. simpl in H0; inversion H0.
+   + inversion H. simpl in H0; inversion H0.
+   + inversion H. simpl in H0; inversion H0.
+   + inversion H. simpl in H0; inversion H0.
+   + inversion H. simpl in H0; inversion H0.
+   + inverts* H.
+    * destruct IHB1; auto.
+      left. apply set_union_intro. left*.
+      destruct H as [x1 [x2]]. destruct H. inversion H.
+    * destruct IHB2; auto.
+      left. apply set_union_intro. right*.
+      destruct H as [x1 [x2]]. destruct H. inversion H.
+    * simpl in H0; inversion H0. 
+   + apply sub_and in H. destruct H.
+     destruct IHB1; auto.
+    * destruct IHB2; auto.
+      left. apply set_inter_intro; auto.
+      destruct H2 as [x1 [x2]]. destruct H2. inversion H2.
+    * destruct H1 as [x1 [x2]]. destruct H1. inversion H1.
+  - induction B; simpl; auto.
+   + inversion H. simpl in H0; inversion H0.
+   + inversion H. simpl in H0; inversion H0.
+   + inversion H. simpl in H0; inversion H0.
+   + inversion H. simpl in H0; inversion H0.
+   + inverts* H.
+    * destruct IHB1; auto.
+      left. apply set_union_intro. left*.
+      destruct H as [x1 [x2]]. destruct H. inversion H.
+    * destruct IHB2; auto.
+      left. apply set_union_intro. right*.
+      destruct H as [x1 [x2]]. destruct H. inversion H.
+    * simpl in H0; inversion H0. 
+   + apply sub_and in H. destruct H.
+     destruct IHB1; auto.
+    * destruct IHB2; auto.
+      left. apply set_inter_intro; auto.
+      destruct H2 as [x1 [x2]]. destruct H2. inversion H2.
+    * destruct H1 as [x1 [x2]]. destruct H1. inversion H1.
+  - induction B; simpl; auto.
+    + inversion H. simpl in H0. inversion H0.
+    + inversion H. simpl in H0; inversion H0.
+    + inversion H. simpl in H0; inversion H0.
+    + inversion H. simpl in H0; inversion H0.
+    + inverts* H.
+     * destruct IHB1; auto.
+       left. apply set_union_intro. left*.
+       destruct H as [x1 [x2]]. destruct H. inversion H.
+     * destruct IHB2; auto.
+       left. apply set_union_intro. right*.
+       destruct H as [x1 [x2]]. destruct H. inversion H.
+     * simpl in H0; inversion H0. 
+    + apply sub_and in H. destruct H.
+      destruct IHB1; auto.
+     * destruct IHB2; auto.
+       left. apply set_inter_intro; auto.
+       destruct H2 as [x1 [x2]]. destruct H2. inversion H2.
+     * destruct H1 as [x1 [x2]]. destruct H1. inversion H1. 
+  - induction B; simpl; auto.
+    + inversion H. simpl in H0. inversion H0.
+    + inversion H. simpl in H0; inversion H0.
+    + inversion H. simpl in H0; inversion H0.
+    + inversion H. simpl in H0; inversion H0.
+    + inverts* H.
+     * destruct IHB1; auto.
+       left. apply set_union_intro. left*.
+       destruct H as [x1 [x2]]. destruct H. inversion H.
+     * destruct IHB2; auto.
+       left. apply set_union_intro. right*.
+       destruct H as [x1 [x2]]. destruct H. inversion H.
+     * simpl in H0; inversion H0. 
+    + apply sub_and in H. destruct H.
+      destruct IHB1; auto.
+     * destruct IHB2; auto.
+       left. apply set_inter_intro; auto.
+       destruct H2 as [x1 [x2]]. destruct H2. inversion H2.
+     * destruct H1 as [x1 [x2]]. destruct H1. inversion H1. 
+  - induction B; simpl; auto.
+   + right. exists* t1 t2.
+   + inversion H. simpl in H0; inversion H0.
+   + inversion H. simpl in H0; inversion H0.
+   + inversion H. simpl in H0; inversion H0.
+   + inversion H. simpl in H0; inversion H0.
+   + right. exists* t1 t2.
+   + inverts* H.
+    * destruct IHB1; auto.
+      left. apply set_union_intro. left*.
+      destruct H as [x1 [x2]]. destruct H.
+      right. exists x1 x2. split*.
+      apply set_union_intro. left*.
+    * destruct IHB2; auto.
+      left. apply set_union_intro. right*.
+      destruct H as [x1 [x2]]. destruct H.
+      right. exists x1 x2. split*.
+      apply set_union_intro. right*.
+    * simpl in H0; inversion H0.
+   + apply sub_and in H. destruct H.
+     destruct IHB1; auto.
+    * destruct IHB2; auto.
+      { left. apply set_inter_intro; auto. }
+      { destruct H2 as [x1 [x2]]. destruct H2.
+        lets H1': H1.
+        apply arrow_in_top_bot in H1'.
+        rewrite <- H1' in H3.
+        left. apply set_inter_intro; auto. }
+    * destruct IHB2; auto.
+      { destruct H1 as [x1 [x2]]. destruct H1.
+        lets H2': H2.
+        apply arrow_in_top_bot in H2'.
+        rewrite <- H2' in H3.
+        left. apply set_inter_intro; auto. }
+      { destruct H1 as [x1 [x2]]. destruct H1.
+        destruct H2 as [x3 [x4]]. destruct H2.
+        right. exists x1 x2. split*.
+        apply set_inter_intro; auto. }
+Defined.
+
+Lemma ord_sub_findsubtypes_not_empty : forall A B, 
+Ord A -> A <: B ->
+(FindSubtypes B) <> [].
+Proof.
+  unfold not. intros.
+  apply ord_in_findsubtypes2 in H0; auto.
+  destruct H0.
+  - rewrite H1 in H0. inversion H0.
+  - destruct H0 as [x1 [x2]]. destruct H0.
+    rewrite H1 in H2. inversion H2.
+Defined.
+
+Lemma list_append_findsubtypes_in : forall t l A, (t :: l) = FindSubtypes A ->
+set_In t (FindSubtypes A).
+Proof.
+  intros.
+  rewrite <- H.
+  apply elem_append_in_list.
+Defined.
+
+Lemma elem_in_findsubtypes_ord : forall A B,
+(set_In B (FindSubtypes A)) -> Ord B.
+Proof.
+  intros.
+  inductions A.
+  - simpl in H.
+    destruct H. rewrite <- H. auto.
+    destruct H. rewrite <- H. auto.
+    destruct H. rewrite <- H. auto.
+    destruct H. rewrite <- H. auto.
+    destruct H. rewrite <- H. auto.
+    inversion H.
+  - simpl in H.
+    destruct H. rewrite <- H. auto.
+    inversion H.
+  - simpl in H.
+    destruct H. rewrite <- H. auto.
+    inversion H.
+  - simpl in H. 
+    destruct H. rewrite <- H. auto.
+    inversion H.
+  - simpl in H. inversion H.
+  - simpl in H.
+    destruct H. rewrite <- H. auto.
+    inversion H.
+  - simpl in H.
+    apply set_union_elim in H. destruct H. 
+    apply IHA1; auto. 
+    apply IHA2; auto.
+  - simpl in H.
+    apply set_inter_elim1 in H.
+    apply IHA1; auto.
+Defined.
+
+
+Lemma inter_not_empty_elim : forall A l,
+l = FindSubtypes A ->
+l <> [] ->
+set_In t_top l \/
+set_In t_int l \/ 
+set_In t_bool l \/
+set_In t_str l \/
+set_In (t_arrow t_top t_bot) l.
+Proof.
+  intros.
+  destruct l.
+  contradiction.
+  lets: elem_append_in_list t l.
+  rewrite H in H1.
+  lets: elem_in_findsubtypes_ord A t. 
+  lets H1': H1.
+  apply H2 in H1.
+  induction H1.
+ - left. apply elem_append_in_list.
+ - right. left. apply elem_append_in_list.
+ - right. right. left. apply elem_append_in_list.
+ - right. right. right. left. apply elem_append_in_list.
+ - apply arrow_in_top_bot in H1'. inverts H1'.
+   right. right. right. right. apply elem_append_in_list.
+Defined.
+
+Lemma not_in5 : forall A B,
+not (set_In t_int (FindSubtypes (t_and A B))) /\
+not (set_In t_bool (FindSubtypes (t_and A B))) /\
+not (set_In t_str (FindSubtypes (t_and A B))) /\
+not (set_In (t_arrow t_top t_bot) (FindSubtypes (t_and A B))) /\
+not (set_In t_top (FindSubtypes (t_and A B))) ->
+(FindSubtypes (t_and A B)) = [].
+Proof.
+  intros.
+  lets: list_empty_decide (FindSubtypes (t_and A B)).
+  destruct H0. 
+  - rewrite H0. auto.
+  - destructs H. 
+    apply inter_not_empty_elim with (A:=(t_and A B)) in H0.
+    destruct H0 as [H5 | [H5 | [H5 | [H5 | H5]]]].
+    contradiction.
+    contradiction.
+    contradiction.
+    contradiction.
+    contradiction.
+    auto.
+Defined.
+
+Lemma demorgan1 : forall P Q : Prop, ~ P /\ ~ Q -> ~ (P \/ Q).
+Proof.
+  intros.
+  destruct H.
+  unfold not in *.
+  intros.
+  destruct H1.
+  apply H; auto.
+  apply H0; auto.
+Defined.
+
+Lemma demorgan2 : forall P Q : Prop, ~ (P \/ Q) -> ~ P /\ ~ Q.
+Proof.
+  intros.
+  unfold not in *.
+  split.
+  intros. apply H. auto.
+  intros. apply H. auto.
+Defined.
+
+Lemma demorgan3 : forall P Q R : Prop, ~ (P \/ Q \/ R) -> ~ P /\ ~ Q /\ ~ R.
+Proof.
+  intros.
+  unfold not in *.
+  split.
+  intros. apply H. auto.
+  split.
+  intros. apply H. auto.
+  intros. apply H. auto.
+Defined.
+
+Lemma demorgan4 : forall P Q R S : Prop, ~ (P \/ Q \/ R \/ S) -> ~ P /\ ~ Q /\ ~ R /\ ~ S.
+Proof.
+  intros.
+  unfold not in *.
+  split.
+  intros. apply H. auto.
+  split.
+  intros. apply H. auto.
+  split.
+  intros. apply H. auto.
+  intros. apply H. auto.
+Defined.
+
+Lemma demorgan5 : forall P Q R S T : Prop, 
+~ (P \/ Q \/ R \/ S \/ T) -> ~ P /\ ~ Q /\ ~ R /\ ~ S /\ ~ T.
+Proof.
+  intros.
+  unfold not in *.
+  splits; intros; apply H; auto.
+Defined.
+
+Lemma elem_in_findsubtypes_sub : forall A B,
+(set_In B (FindSubtypes A)) -> B <: A.
+Proof.
+  intros.
+  inductions A.
+  - simpl in H.
+    destruct H as [H | [H | [H | [H | [H | H] ] ] ] ]; 
+    try solve [rewrite <- H; auto].
+    inversion H.
+  - simpl in H.
+    destruct H. rewrite <- H. auto.
+    inversion H.
+  - simpl in H.
+    destruct H. rewrite <- H. auto.
+    inversion H.
+  - simpl in H.
+    destruct H. rewrite <- H. auto.
+    inversion H. 
+  - simpl in H. inversion H.
+  - simpl in H.
+    destruct H. rewrite <- H. auto.
+    inversion H.
+  - simpl in H.
+    apply set_union_elim in H. destruct H. 
+    apply s_orb. apply IHA1; auto. 
+    apply s_orc. apply IHA2; auto.
+  - simpl in H.
+    apply s_anda.
+    apply set_inter_elim1 in H. 
+    apply IHA1; auto.
+    apply set_inter_elim2 in H. 
+    apply IHA2; auto.
+Defined.
+
+
+Lemma findsubtypes_empty_not_ord : forall A B,
+FindSubtypes A = [] -> B <: A -> not (Ord B).
+Proof.
+    intros.
+    unfold not. intros.
+    lets: ord_in_findsubtypes2 B A.
+    inverts H1.
+    - destruct H2; auto.
+      rewrite H in H1. inverts H1.
+      destruct H1 as [x1 [x2]].
+      destruct H1. inversion H1.
+    - destruct H2; auto.
+      rewrite H in H1. inverts H1.
+      destruct H1 as [x1 [x2]].
+      destruct H1. inversion H1.
+    - destruct H2; auto.
+      rewrite H in H1. inverts H1.
+      destruct H1 as [x1 [x2]].
+      destruct H1. inversion H1.
+    - destruct H2; auto.
+      rewrite H in H1. inverts H1.
+      destruct H1 as [x1 [x2]].
+      destruct H1. inversion H1.
+    - destruct H2; auto.
+      rewrite H in H1. simpl in H1. inversion H1.
+      destruct H1 as [x1 [x2]]. destruct H1.
+      rewrite H in H2. simpl in H2. inversion H2.
+Defined.
+
+Lemma findsubtypes_empty_no_ord_sub1 : forall A1 A2,
+FindSubtypes (t_and A1 A2) = [] -> 
+not (exists B, Ord B /\ B <: (t_and A1 A2)).
+Proof.
+  unfold not. intros.
+  destruct H0. destruct H0.
+  lets: ord_sub_findsubtypes_not_empty x (t_and A1 A2) H0 H1.
+  contradiction.
+Defined.
+
+Lemma findsubtypes_empty_no_ord_sub2 : forall A1 A2,
+FindSubtypes (t_and A1 A2) = [] -> 
+forall B, Ord B -> not(B <: (t_and A1 A2)).
+Proof.
+  unfold not. intros.
+  lets: ord_sub_findsubtypes_not_empty B (t_and A1 A2) H1. auto.
+  contradiction.
+Defined.
+
+Lemma no_ord_sub_not_in : forall A1 A2,
+forall B, Ord B -> not(B <: (t_and A1 A2)) ->
+not (set_In B (FindSubtypes (t_and A1 A2))).
+Proof.
+  intros. unfold not. intros.
+  apply elem_in_findsubtypes_sub in H1.
+  contradiction.
+Defined.
+
+Lemma findsubtypes_not_empty : forall A,
+FindSubtypes A <> [] -> exists B, set_In B (FindSubtypes A).
+Proof.
+  intros.
+  destruct (FindSubtypes A).
+  contradiction.
+  lets: elem_append_in_list t l.
+  exists t. auto.
+Defined.
+
+Lemma not_ord_sub_not_in : forall A, not (Ord A) ->
+forall B, Ord B -> not (B <: A) -> not (set_In B (FindSubtypes A)).
+Proof.
+intros.
+unfold not in *. intros.
+lets: elem_in_findsubtypes_sub A B H2.
+contradiction.
+Defined.
+
+Lemma set_in_sub : forall A x, set_In x (FindSubtypes A) ->
+forall B, A <: B -> set_In x (FindSubtypes B).
+Proof.
+  intros.
+  inductions H0; eauto.
+  - lets H': H.
+    apply elem_in_findsubtypes_ord in H'.
+    simpl. destruct H'.
+    right. right. auto.
+    left. auto.
+    right. left. auto.
+    right. right. auto.
+    apply arrow_in_top_bot in H.
+    rewrite H. auto.
+  - simpl in H. apply set_union_elim in H.
+    destruct H. 
+    apply IHsubtyping1; auto.
+    apply IHsubtyping2; auto.
+  - simpl. apply set_union_intro1. apply IHsubtyping; auto.
+  - simpl. apply set_union_intro2. apply IHsubtyping; auto.
+  - simpl. apply set_inter_intro.
+    apply IHsubtyping1; auto.
+    apply IHsubtyping2; auto.
+  - simpl in H. apply set_inter_elim1 in H.
+    apply IHsubtyping; auto.
+  - simpl in H. apply set_inter_elim2 in H.
+    apply IHsubtyping; auto.
+  - rewrite H0 in H.
+    inverts H.
+Defined.
+
+Lemma findsubtypes_sub_empty : forall A1 A2 B,
+FindSubtypes (t_and A1 A2) = [] -> 
+B <: (t_and A1 A2) -> FindSubtypes B = [].
+Proof.
+    intros.
+    lets: list_empty_decide (FindSubtypes B).
+    destruct H1. auto.
+    lets: findsubtypes_not_empty B H1.
+    destruct H2.
+    lets: set_in_sub B x H2 (t_and A1 A2) H0.
+    rewrite H in H3. inverts H3.
+Defined.
+
 Lemma sub_refl : forall A, A <: A.
   induction A; eauto.
 Defined.
 
 Hint Resolve sub_refl.
-
 
 Lemma sub_transitivity : forall B A C, A <: B -> B <: C -> A <: C.
 Proof.
@@ -259,141 +833,78 @@ generalize H0 H; clear H0; clear H; generalize A; clear A.
 - intros; inductions H0; eauto. 
 - intros; inductions H; eauto.
 - intros; inductions H; eauto.
-- induction C; intros; inverts* H0.
-  induction A; inverts* H.
+- intros; inductions H; eauto.
+- intros; inductions H; eauto.
+- induction C; intros; try solve [inverts* H0].
+  inverts H0. inverts H1.
+  inverts H0. inverts H1.
+  inverts H0. inverts H1.
+  inverts H0. inverts H1.
+  induction A; try solve[inverts* H].
+  inverts* H0. inverts* H. 
 - intros. apply sub_or in H0. destruct H0.
   inductions H; eauto.
 - intros. apply sub_and in H. destruct H.
   inductions H0; eauto.
+  assert (A <: t_and B1 B2) by auto.
+  apply s_disj.
+  apply findsubtypes_sub_empty with (A1:=B1) (A2:=B2). auto. auto.
 Defined.
 
-
-(*************************)
-(***** Ordinary Types ****)
-(*************************)
-
-Inductive Ord : typ -> Prop :=
-| o_top : Ord typ_top
-| o_int : Ord t_int
-| o_arrow : forall t1 t2, Ord (t_arrow t1 t2).
-(*| o_union : forall t1 t2, Ord t1 -> Ord t2 -> Ord (t_union t1 t2).*)
-
-Hint Constructors Ord.
-
-(****************************************)
-(*********  Bottom-Like Specs   *********)
-(****************************************)
-
- (*Definition btmLikeSpec C := (exists A B, 
- Isomorphic (t_and A B) C -> (not (A <: B) /\ not (B <: A))) \/
-C <: t_bot.*)
-
-Definition btmLikeSpec C := forall A, Ord A -> not (A <: C).
-
-(*Definition btmLikeSpec C := (forall A B,  Isomorphic (t_and A B) C -> 
-btmLikeSpec A \/ btmLikeSpec B \/ (not (A <: B) /\ not (B <: A))) \/ C <: t_bot.*)
+Lemma bot_sub_all : forall A, t_bot <: A.
+Proof.
+  intros.
+  dependent induction A; eauto.
+Qed.
 
 (****************************************)
 (**********  Dijoint Specs    ***********)
 (****************************************)
 
-Definition DisjSpec A B := forall C, C <: A /\ C <: B -> btmLikeSpec C.
+(*
 
+A *s B = not (exists C, Ord C -> C <: A /\ C <: B)
+
+*)
+
+Definition DisjSpec A B := forall C, Ord C -> not (C <:  (t_and A B)).
 Notation "A *s B" := (DisjSpec A B) (at level 80).
 
-(* defns BottomLike *)
+(****************************************)
+(**********  Dijoint Algo    ************)
+(****************************************)
 
-Reserved Notation "A *a B" (at level 80).
+(*
+Eval compute in (FindSubtypes t_int).
+Eval compute in (FindSubtypes (t_and t_int t_bot)).
+Eval compute in (FindSubtypes (t_and t_int t_top)).
+Eval compute in (FindSubtypes (t_and t_top t_int)).
+Eval compute in (FindSubtypes (t_and (t_arrow t_int t_int) t_int)).
+Eval compute in (FindSubtypes (t_and(t_and (t_arrow t_int t_int) t_int)t_top)).
+Eval compute in (FindSubtypes (t_and t_top(t_and (t_arrow t_int t_int) t_int))).
+Eval compute in (FindSubtypes (t_union (t_and t_top(t_and (t_arrow t_int t_int) t_int)) (t_and t_top(t_and (t_arrow t_int t_int) t_int)))).
+Eval compute in (FindSubtypes (t_and (t_union t_top(t_union (t_arrow t_int t_int) t_int)) (t_union t_top(t_union (t_arrow t_int t_int) t_int)))).
+Eval compute in (FindSubtypes (t_and t_top t_bot)).
+Eval compute in (FindSubtypes (t_and (t_arrow t_int t_int) (t_arrow (t_arrow t_int t_int) t_int))).
+Eval compute in (FindSubtypes (t_union t_int t_bot)).
+Eval compute in (FindSubtypes (t_and (t_union t_int (t_arrow t_int t_int)) t_int)).
+Eval compute in (FindSubtypes (t_union t_int (t_arrow t_int t_int))).
+Eval compute in (FindSubtypes (t_and (t_arrow t_int t_int) t_top)).
+Eval simpl in (FindSubtypes (t_and t_top (t_arrow t_int t_int))).
+*)
 
-Inductive bottomlike : typ -> Prop :=    (* defn bottomlike *)
- | bl_bot :
-     bottomlike t_bot
- | bl_or : forall (A B:typ),
-     bottomlike A ->
-     bottomlike B ->
-     bottomlike (t_union A B)
- | bl_anda : forall A B,
-     bottomlike A ->
-     bottomlike (t_and A B)
- | bl_andb : forall A B,
-     bottomlike B ->
-     bottomlike (t_and A B)
- | bl_andsub : forall A B,
-     A *a B ->
-     bottomlike (t_and A B)
-
-(* defns Disjointness *)
-with disjointness : typ -> typ -> Prop :=    (* defn disjointness *)
- | ad_btml : forall (A B:typ),
-      bottomlike A ->
-      A *a B
- | ad_btmr : forall (A B:typ),
-     bottomlike B ->
-     A *a B
- | ad_intl : forall (A B:typ),
-     t_int *a (t_arrow A B)
- | ad_intr : forall (A B:typ),
-     (t_arrow A B) *a t_int
- | ad_orl : forall (A B C:typ),
-     A *a C ->
-     B *a C ->
-     (t_union A B) *a C
- | ad_orr : forall (A B C:typ),
-     A *a B ->
-     A *a C ->
-     A *a (t_union B C)
- | ad_andl1 : forall A B C,
-     A *a C ->
-     (t_and A B) *a C
- | ad_andl2 : forall A B C,
-     B *a C ->
-     (t_and A B) *a C
- | ad_andr1 : forall A B C,
-     A *a B ->
-     A *a (t_and B C)
- | ad_andr2 : forall A B C,
-     (*A *a C ->*)
-     A *a C ->
-     A *a (t_and B C)
-
-where "A *a B" := (disjointness A B).
-
-Hint Constructors disjointness.
-
-Hint Constructors bottomlike.
-
-(*Scheme bottomlike_disjointness := Minimality for bottomlike Sort Prop
-with disjointness_bottomlike := Minimality for disjointness Sort Prop.*)
+Definition DisjAlgo A B := ((FindSubtypes A) `inter` (FindSubtypes B)) = [].
+Notation "A *a B" := (DisjAlgo A B) (at level 80).
 
 (**********************************)
-(****  Bottom-Like Properties  ****)
+(****  DisjSpec Properties  ****)
 (**********************************)
 
 Lemma ord_sub_bot_false : forall A, Ord A -> A <: t_bot -> False.
 Proof.
   intros.
-  dependent induction H; inversion H0.
-Defined.
-
-
-Lemma btm_sub_btmlike : forall A, A <: t_bot -> bottomlike A.
-Proof.
-intros. inductions H; eauto.
-Defined.
-
-Lemma btm_sub_btmlikeSpec : forall A, A <: t_bot -> btmLikeSpec A.
-Proof.
-intros. unfold btmLikeSpec. unfold not. intros.
-eapply sub_transitivity in H; eauto.
-forwards*: ord_sub_bot_false H0.
-Defined.
-
-
-Lemma btm_like_and : forall A B, bottomlike (t_and A B) ->
-bottomlike A \/ bottomlike B \/ A *a B.
-Proof.
-  intros.
-  dependent induction H; eauto.
+  dependent induction H; inversion H0;
+  simpl in H; inversion H.
 Defined.
 
 Lemma not_sub_and : forall A1 A2, forall A, Ord A ->
@@ -404,23 +915,6 @@ Proof.
   apply H0; destruct~ H1.
 Defined.
 
-Lemma btm_like_spec_and : forall A1 A2, btmLikeSpec (t_and A1 A2) ->
-  A1 *s A2.
-Proof.
-  intros.
-  unfold btmLikeSpec in *.
-  unfold DisjSpec.
-  intros.
-  destruct H0.
-  unfold btmLikeSpec.
-  intros.
-  unfold not in *.
-  intros.
-  eapply H; eauto.
-  assert (C <: (t_and A1 A2)) by auto.
-  eapply sub_transitivity in H4; eauto.
-Defined.
-
 Lemma ord_sub_and_or : forall B C, forall A, Ord A ->
 not (A <: (t_and B C)) -> not(A <: B) \/ not(A <: C) \/ not (A <: (t_and B C)).
 Proof.
@@ -428,12 +922,480 @@ Proof.
   unfold not in *. auto.
 Defined.
 
+Lemma not_sub_or_inv : forall A A1 A2, Ord A -> not (A <: A1) -> not (A <: A2) -> not (A <: (t_union A1 A2)).
+Proof.
+  intros.
+  unfold not in *.
+  intros. inductions H; inverts* H2.
+Defined.
+
+Lemma btm_sub : forall A, t_bot <: A.
+Proof.
+  intros; auto.
+Defined.
+
+Lemma ord_sub_union : forall A, Ord A -> forall A1 A2, A <: t_union A1 A2 -> A <: A1 \/ A <: A2.
+Proof.
+  intros A H.
+  dependent induction H; intros;
+  inverts* H.
+Defined.
+
+Lemma not_sub_and1_inv : forall A A1 A2, Ord A -> not (A <: A1) -> not (A <: (t_and A1 A2)).
+Proof.
+  intros.
+  unfold not in *.
+  intros. inductions H; inverts* H1.
+Defined.
+
+Lemma not_sub_and2_inv : forall A A1 A2, Ord A -> not (A <: A2) -> not (A <: (t_and A1 A2)).
+Proof.
+  intros.
+  unfold not in *.
+  intros. inductions H; inverts* H1.
+Defined.
+
+Lemma disj_union_intro : forall A B C, A *s C -> B *s C -> t_union A B *s C.
+Proof.
+  intros.
+  unfold DisjSpec in *. intros.
+  unfold not in *. intros.
+  specialize (H C0).
+  apply H; auto.
+  apply sub_and in H2.
+  destruct H2.
+  lets: ord_sub_union C0 H1 A B H2.
+  destruct H4.
+  apply s_anda; auto.
+  specialize (H0 C0).
+  forwards*: H0.
+Defined.
+
+Lemma disj_union_elim : forall A B C, A *s t_union B C -> A *s B /\ A *s C.
+Proof.
+  unfold DisjSpec; unfold not; intros.
+  split.
+  - intros. apply sub_and in H1. destruct H1.
+    specialize (H C0).
+    apply H; auto.
+  - intros. apply sub_and in H1. destruct H1.
+    specialize (H C0).
+    apply H; auto.
+Defined.
+
+Lemma ord_sub_disj_spec_false : forall A, Ord A -> 
+forall B C, B *s C -> A <: (t_and B C) -> False.
+Proof.
+ unfold DisjSpec; unfold not; intros.
+ apply sub_and in H1. destruct H1.
+ specialize (H0 A).
+ forwards*: H0 H.
+Defined.
+
+Lemma Disj_sym_spec : forall A B, A *s B -> B *s A.
+Proof.
+  unfold DisjSpec; unfold not; intros.
+  intros.
+  forwards*: H H0.
+  apply sub_and in H1. destruct H1.
+  apply s_anda; auto.
+Defined.
+
+Lemma ord_bot : Ord t_bot -> False.
+Proof.
+  inversion 1.
+Defined.
+
+Lemma ord_and : forall A B, Ord (t_and A B) -> False.
+Proof.
+  inversion 1.
+Defined.
+
+Lemma ord_union : forall A B, Ord (t_union A B) -> False.
+Proof.
+  inversion 1.
+Defined.
+
+(*
+Below lemma states that all the elements of FindSubtypes are ordinary.
+*)
+
+Lemma ord_findsubtypes_not_empty : forall A,
+Ord A -> (FindSubtypes A) <> [].
+Proof.
+  intros A H.
+  induction A; unfold not; intros; 
+  try solve [simpl in H0; inversion H0; inversion H].
+Defined.
+
+Lemma union_findsubtypes_empty_intro : forall A B,
+(FindSubtypes A = []) -> (FindSubtypes B = []) ->
+((FindSubtypes A) `union` (FindSubtypes B)) = [].
+Proof.
+  intros.
+  induction (FindSubtypes A).
+  - rewrite H0. simpl. auto.
+  - inversion H.
+Defined.
+
+(*  
+**************************************************************
+Another approach to prove ord_sub_findsubtypes_not_empty lemma
+**************************************************************
+
+  intros A B H. gen B.
+  induction B; unfold not; intros H1 H2; 
+  try solve [simpl in H2; inversion H2].
+  - apply ord_sub_bot_false in H1; auto.
+  - (*apply union_findsubtypes_empty_elim in H2. destruct H2.
+    apply ord_sub_union in H1; auto. destruct H1.
+    unfold not in IHB1; apply IHB1; auto.
+    unfold not in IHB2; apply IHB2; auto.*)
+    apply ord_in_findsubtypes2 in H1; auto.
+    destruct H1.
+    rewrite H2 in H0. inversion H0.
+    destruct H0 as [x1 [x2]]. destruct H0.
+    rewrite H2 in H1. inversion H1.
+  - apply ord_in_findsubtypes2 in H1; auto.
+    destruct H1.
+    rewrite H2 in H0. inversion H0.
+    destruct H0 as [x1 [x2]]. destruct H0.
+    rewrite H2 in H1. inversion H1.
+Defined.
+*)
+
+Lemma Disj_soundness : forall A B, A *a B -> A *s B.
+Proof.
+(* Disj_soundness Soundness Proof *)
+intros.
+unfold DisjAlgo in H.
+unfold DisjSpec. unfold not. intros.
+apply ord_sub_findsubtypes_not_empty in H1; auto.
+Qed.
+
+Definition DisjSpec1 A B := not (exists C, Ord C /\ C <: (t_and A B)).
+Notation "A *s1 B" := (DisjSpec1 A B) (at level 80).
+
+Lemma disj_disj1 : forall A B, A *s B -> A *s1 B.
+Proof.
+  unfold DisjSpec. unfold DisjSpec1. unfold not. intros.
+  destruct H0. destruct H0.
+  specialize (H x).
+  apply H; auto.
+Defined.
+
+Lemma disj1_disj : forall A B, A *s1 B -> A *s B.
+Proof.
+  unfold DisjSpec. unfold DisjSpec1. unfold not. intros.
+  apply H. exists* C.
+Defined.
+
+Lemma exists_inter_empty : exists B C,
+(FindSubtypes B `inter` FindSubtypes C) = [].
+Proof.
+  exists t_int (t_arrow t_top t_bot).
+  simpl. auto.
+Defined.
+
+Lemma decidability: forall A B, Ord A -> 
+(set_In A (FindSubtypes B)) \/ ~(set_In A (FindSubtypes B)) \/
+(exists t1 t2, A = t_arrow t1 t2 /\ set_In (t_arrow t_top t_bot) (FindSubtypes B)).
+Proof.
+  induction A; try solve [intros; inversion H].
+  - intros. induction B; auto.
+   + left. simpl. right. auto.
+   + right. left. simpl. unfold not. 
+     intros. inverts* H0. inverts* H1.
+   + right. left. unfold not. intros.
+     simpl in H0. destruct H0; inversion H0.
+   + right. left. simpl. unfold not. 
+     intros. inverts* H0. inverts* H1.
+   + right. left. simpl. unfold not. 
+     intros. inverts* H0. inverts* H1.
+   + destruct IHB1. 
+     left. simpl. apply set_union_intro1. auto.
+     destruct IHB2. 
+     left. simpl. apply set_union_intro2. auto.
+     destruct H0. destruct H1. 
+     right. left. unfold not in *. intros.
+     simpl in H2. apply set_union_elim in H2.
+     destruct H2. apply H0; auto. apply H1; auto.
+     destruct H1 as [x1 [x2]]. destruct H1. inversion H1.
+     destruct H0 as [x1 [x2]]. destruct H0. inversion H0.
+   + destruct IHB1. destruct IHB2.
+     left. simpl. apply set_inter_intro; auto.
+     destruct H1. 
+     right. left. unfold not in *.
+     intros. simpl in H2. apply H1.
+     apply set_inter_elim2 in H2. auto.
+     destruct H1 as [x1 [x2]]. destruct H1. inversion H1.
+     destruct H0. 
+     right. left. unfold not in *. 
+     intros. simpl in H1. apply H0.
+     apply set_inter_elim1 in H1. auto.
+     destruct H0 as [x1 [x2]]. destruct H0. inversion H0.
+  - intros. induction B; auto.
+   + left. simpl. auto.
+   + left. simpl. auto.
+   + right. left. unfold not. simpl.
+     intros. destruct H0; inversion H0.
+   + right. left. unfold not. simpl.
+     intros. destruct H0; inversion H0. 
+   + right. left. simpl. unfold not. 
+     intros. inverts* H0. inverts* H1.
+   + destruct IHB1. 
+     left. simpl. apply set_union_intro1. auto.
+     destruct IHB2. 
+     left. simpl. apply set_union_intro2. auto.
+     destruct H0. destruct H1. 
+     right. left. unfold not in *. intros.
+     simpl in H2. apply set_union_elim in H2.
+     destruct H2. apply H0; auto. apply H1; auto.
+     destruct H1 as [x1 [x2]]. destruct H1. inversion H1.
+     destruct H0 as [x1 [x2]]. destruct H0. inversion H0.
+   + destruct IHB1. destruct IHB2.
+     left. simpl. apply set_inter_intro; auto.
+     destruct H1. 
+     right. left. unfold not in *.
+     intros. simpl in H2. apply H1.
+     apply set_inter_elim2 in H2. auto.
+     destruct H1 as [x1 [x2]]. destruct H1. inversion H1.
+     destruct H0. 
+     right. left. unfold not in *. 
+     intros. simpl in H1. apply H0.
+     apply set_inter_elim1 in H1. auto.
+     destruct H0 as [x1 [x2]]. destruct H0. inversion H0.
+  - intros. induction B; auto.
+   + left. simpl. auto.
+   + right. left. simpl. unfold not. intros.
+     destruct H0; inversion H0.
+   + left. simpl. auto.
+   + right. left. unfold not. simpl.
+     intros. destruct H0; inversion H0.
+   + right. left. simpl. unfold not. 
+     intros. inverts* H0. inverts* H1.
+   + destruct IHB1. 
+     left. simpl. apply set_union_intro1. auto.
+     destruct IHB2. 
+     left. simpl. apply set_union_intro2. auto.
+     destruct H0. destruct H1. 
+     right. left. unfold not in *. intros.
+     simpl in H2. apply set_union_elim in H2.
+     destruct H2. apply H0; auto. apply H1; auto.
+     destruct H1 as [x1 [x2]]. destruct H1. inversion H1.
+     destruct H0 as [x1 [x2]]. destruct H0. inversion H0.
+   + destruct IHB1. destruct IHB2.
+     left. simpl. apply set_inter_intro; auto.
+     destruct H1. 
+     right. left. unfold not in *.
+     intros. simpl in H2. apply H1.
+     apply set_inter_elim2 in H2. auto.
+     destruct H1 as [x1 [x2]]. destruct H1. inversion H1.
+     destruct H0. 
+     right. left. unfold not in *. 
+     intros. simpl in H1. apply H0.
+     apply set_inter_elim1 in H1. auto.
+     destruct H0 as [x1 [x2]]. destruct H0. inversion H0.
+  - intros. induction B; auto.
+   + left. simpl. auto.
+   + right. left. simpl. unfold not. intros.
+     destruct H0; inversion H0.
+   + right. left. simpl. unfold not.
+     intros. destruct H0; inversion H0.
+   + left. simpl. auto.
+   + right. left. simpl. unfold not. 
+     intros. inverts* H0. inverts* H1.
+   + destruct IHB1. 
+     left. simpl. apply set_union_intro1. auto.
+     destruct IHB2. 
+     left. simpl. apply set_union_intro2. auto.
+     destruct H0. destruct H1. 
+     right. left. unfold not in *. intros.
+     simpl in H2. apply set_union_elim in H2.
+     destruct H2. apply H0; auto. apply H1; auto.
+     destruct H1 as [x1 [x2]]. destruct H1. inversion H1.
+     destruct H0 as [x1 [x2]]. destruct H0. inversion H0.
+   + destruct IHB1. destruct IHB2.
+     left. simpl. apply set_inter_intro; auto.
+     destruct H1. 
+     right. left. unfold not in *.
+     intros. simpl in H2. apply H1.
+     apply set_inter_elim2 in H2. auto.
+     destruct H1 as [x1 [x2]]. destruct H1. inversion H1.
+     destruct H0. 
+     right. left. unfold not in *. 
+     intros. simpl in H1. apply H0.
+     apply set_inter_elim1 in H1. auto.
+     destruct H0 as [x1 [x2]]. destruct H0. inversion H0.
+  - intros. induction B; auto.
+   + right. right. exists A1 A2. split*.
+     simpl. auto.
+   + right. left. simpl. unfold not. 
+     intros. inverts* H0. inverts* H1.
+   + right. left. unfold not. simpl. intros.
+     destruct H0; inversion H0.
+   + right. left. unfold not. simpl.
+     intros. destruct H0; inversion H0.
+   + right. right. simpl. exists A1 A2. split*.
+   + destruct IHB1. 
+     left. simpl. apply set_union_intro1. auto.
+     destruct IHB2. 
+     left. simpl. apply set_union_intro2. auto.
+     destruct H0. destruct H1. 
+     right. left. unfold not in *. intros.
+     simpl in H2. apply set_union_elim in H2.
+     destruct H2. apply H0; auto. apply H1; auto.
+     destruct H1 as [x1 [x2]]. destruct H1.
+     right. right. exists A1 A2. split*.
+     simpl. apply set_union_intro. right*.
+     destruct H0 as [x1 [x2]]. destruct H0.
+     right. right. exists A1 A2. split*.
+     simpl. apply set_union_intro. left*.
+   + destruct IHB1. destruct IHB2.
+     left. simpl. apply set_inter_intro; auto.
+     destruct H1. 
+     right. left. unfold not in *.
+     intros. simpl in H2. apply H1.
+     apply set_inter_elim2 in H2. auto.
+     destruct H1 as [x1 [x2]]. destruct H1.
+     right. right. exists A1 A2. split*.
+     lets H0': H0.
+     apply arrow_in_top_bot in H0'. inverts H0'.
+     simpl. apply set_inter_intro; auto.
+     destruct H0. 
+     right. left. unfold not in *. 
+     intros. simpl in H1. apply H0.
+     apply set_inter_elim1 in H1. auto.
+     destruct H0 as [x1 [x2]]. destruct H0.
+     destruct IHB2.
+     lets H2': H2. apply arrow_in_top_bot in H2'. inverts H2'.
+     left. simpl. apply set_inter_intro; auto.
+     destruct H2.
+     right. left. unfold not in *. intros.
+     apply H2. simpl in H3. apply set_inter_elim2 in H3. auto.
+     destruct H2 as [x3 [x4]]. destruct H2.
+     right. right. exists A1 A2. split*.
+     simpl. apply set_inter_intro; auto.
+Defined.
+
+Lemma not_in_inter_intro1 : forall A B, not (set_In A (FindSubtypes B)) ->
+forall C, not (set_In A (FindSubtypes B `inter` FindSubtypes C)).
+Proof.
+  unfold not in *. intros.
+  apply set_inter_elim1 in H0; apply H; auto.
+Defined.
+
+Lemma not_in_inter_intro2 : forall A C, not (set_In A (FindSubtypes C)) ->
+forall B, not (set_In A (FindSubtypes B `inter` FindSubtypes C)).
+Proof.
+  unfold not in *. intros.
+  apply set_inter_elim2 in H0; apply H; auto.
+Defined.
+
+Lemma not_in_union_elim : forall A B C, 
+not (set_In A (FindSubtypes (t_union B C))) ->
+not (set_In A (FindSubtypes B)) /\ not (set_In A (FindSubtypes C)).
+Proof.
+  unfold not in *. intros.
+  split; intros.
+  apply H. simpl. apply set_union_intro1. auto.
+  apply H. simpl. apply set_union_intro2. auto.
+Defined.
+
+Definition DisjAlgo1 A B := (FindSubtypes (t_and A B)) = [].
+Notation "A *a1 B" := (DisjAlgo1 A B) (at level 80).
+
+Lemma disja_disja1 : forall A B, DisjAlgo A B -> DisjAlgo1 A B.
+Proof.
+  unfold DisjAlgo.
+  unfold DisjAlgo1.
+  intros. simpl. auto.
+Defined.
+
+Lemma disja1_disja : forall A B, DisjAlgo1 A B -> DisjAlgo A B.
+Proof.
+  unfold DisjAlgo.
+  unfold DisjAlgo1.
+  intros. simpl in H. auto.
+Defined.
+
+Lemma Disj_completeness2 : forall A B,  A *s B -> A *a1 B.
+Proof.
+  intros.
+  apply disj_disj1 in H.
+  unfold DisjSpec1 in H. unfold not in H.
+  unfold DisjAlgo1.
+  eapply not_in5.
+  apply demorgan5. unfold not. intros.
+  destruct H0 as [H1 | [H1 | [H1 | [H1 | H1]]]];
+  lets H1': H1;
+  apply elem_in_findsubtypes_sub in H1';
+  lets H1'': H1;
+  apply elem_in_findsubtypes_ord in H1'';
+  apply H. 
+ - exists t_int. split*.
+ - exists t_bool. split*.
+ - exists t_str. split*.
+ - exists (t_arrow t_top t_bot). split*.
+ - exists t_top. split*.
+(* 
+
+longer way to prove completeness:
+
+- lets H1': H1.
+  apply elem_in_findsubtypes_sub in H1'.
+  lets H1'': H1.
+  apply elem_in_findsubtypes_ord in H1''.
+  apply H. exists t_bool. split*.
+- lets H1': H1.
+  apply elem_in_findsubtypes_sub in H1'.
+  lets H1'': H1.
+  apply elem_in_findsubtypes_ord in H1''.
+  apply H. exists t_bool. split*.
+- lets H1': H1.
+   apply elem_in_findsubtypes_sub in H1'.
+  lets H1'': H1.
+  apply elem_in_findsubtypes_ord in H1''.
+  apply H. exists (t_arrow t_top t_bot). split*.
+-  lets H1': H1.
+  apply elem_in_findsubtypes_sub in H1'.
+  lets H1'': H1.
+  apply elem_in_findsubtypes_ord in H1''.
+  apply H. exists t_top. split*.
+  *)
+Qed.
+
+Lemma Disj_completeness3 : forall A B,  A *s B -> A *a B.
+Proof.
+  intros.
+  unfold DisjSpec in H. unfold not in H.
+  unfold DisjAlgo.
+  eapply not_in5.
+  apply demorgan5. unfold not. intros.
+  destruct H0 as [H1 | [H1 | [H1 | [H1 | H1]]]];
+  lets H1': H1;
+  apply elem_in_findsubtypes_sub in H1';
+  lets H1'': H1;
+  apply elem_in_findsubtypes_ord in H1''.
+  eapply H; eauto.
+  eapply H; eauto.
+  eapply H; eauto.
+  eapply H; eauto.
+  eapply H; eauto.
+Qed.
+
 
 (* defns Typing *)
 Inductive typing : env -> exp -> dirflag -> typ -> Prop :=    (* defn typing *)
  | typ_lit : forall (G:env) i5,
       okt  G  ->
      typing G (e_lit i5) infer t_int
+ | typ_bool : forall (G:env) b,
+      okt  G  ->
+     typing G (e_bool b) infer t_bool
+ | typ_str : forall (G:env) s,
+      okt G ->
+      typing G (e_str s) infer t_str
  | typ_var : forall (G:env) (x:var) (A:typ),
       okt  G  ->
       binds  x A G  ->
@@ -466,6 +1428,10 @@ Reserved Notation "e --> e'" (at level 80).
 Inductive step : exp -> exp -> Prop :=    (* defn step *)
  | step_int : forall i5,
      step (e_lit i5) (e_ann (e_lit i5) t_int)
+ | step_bool : forall b,
+     step (e_bool b) (e_ann (e_bool b) t_bool)
+ | step_str : forall s,
+     step (e_str s) (e_ann (e_str s) t_str)
  | step_appl : forall (e1 e2 e1':exp),
      lc_exp e2 ->
      step e1 e1' ->
@@ -511,1217 +1477,3 @@ Inductive step : exp -> exp -> Prop :=    (* defn step *)
 where "e --> e'" := (step e e') : env_scope.
 
 Hint Constructors step.
-
-(*************************************)
-(*****  Disjointness Properties  *****)
-(*************************************)
-
-(** infrastructure *)
-
-Lemma not_sub_or_inv : forall A A1 A2, Ord A -> not (A <: A1) -> not (A <: A2) -> not (A <: (t_union A1 A2)).
-Proof.
-  intros.
-  unfold not in *.
-  intros. inductions H; inverts* H2.
-Defined.
-
-Lemma btm_like_spec_union_inv : forall A B, btmLikeSpec A -> btmLikeSpec B -> btmLikeSpec (t_union A B).
-Proof.
-  intros.
-  unfold btmLikeSpec in *.
-  intros.
-  lets: H A0 H1.
-  lets: H0 A0 H1.
-  apply* not_sub_or_inv.
-Defined.
-
-Lemma btm_sub : forall A, t_bot <: A.
-Proof.
-  intros; auto.
-Defined.
-
-Lemma not_sub_and1_inv : forall A A1 A2, Ord A -> not (A <: A1) -> not (A <: (t_and A1 A2)).
-Proof.
-  intros.
-  unfold not in *.
-  intros. inductions H; inverts* H1.
-Defined.
-
-Lemma not_sub_and2_inv : forall A A1 A2, Ord A -> not (A <: A2) -> not (A <: (t_and A1 A2)).
-Proof.
-  intros.
-  unfold not in *.
-  intros. inductions H; inverts* H1.
-Defined.
-
-Lemma btm_like_spec_and1_inv : forall A B, btmLikeSpec A -> btmLikeSpec (t_and A B).
-Proof.
-  intros.
-  unfold btmLikeSpec in *.
-  intros.
-  lets: H A0 H0.
-  apply* not_sub_and1_inv.
-Defined.
-
-Lemma btm_like_spec_and2_inv : forall A B, btmLikeSpec B -> btmLikeSpec (t_and A B).
-Proof.
-  intros.
-  unfold btmLikeSpec in *.
-  intros.
-  lets: H A0 H0.
-  apply* not_sub_and2_inv.
-Defined.
-
-Lemma btm_spec : btmLikeSpec t_bot.
-Proof.
-  unfold btmLikeSpec.
-  intros.
-  unfold not.
-  intros.
-  inductions H; inverts* H0.
-Defined.
-
-Lemma ord_sub_union : forall A, Ord A -> forall A1 A2, A <: t_union A1 A2 -> A <: A1 \/ A <: A2.
-Proof.
-  intros A H.
-  dependent induction H; intros.
-  inverts* H.
-  inverts* H.
-  inverts* H.
-Defined.
-
-Lemma btm_like_spec_btm_inter : forall A, btmLikeSpec (t_and A t_bot).
-Proof.
-  intros.
-  unfold btmLikeSpec. intros.
-  unfold not. intros.
-  apply sub_and in H0.
-  destruct H0.
-  apply ord_sub_bot_false in H1; auto.
-Defined.
-
-
-Lemma sub_int_arrow : forall A B, A <: t_int -> forall A1 A2, B <: (t_arrow A1 A2) -> btmLikeSpec (t_and A B).
-Proof.
-  intros.
-  inductions H.
-  - apply* btm_like_spec_and1_inv. apply btm_spec.
-  - inductions H0.
-   + apply btm_like_spec_btm_inter.
-   + unfold btmLikeSpec. intros.
-     unfold not. intros.
-     inverts* H; inverts* H0. inversion H3. inversion H4. inversion H3.
-   + forwards*: IHsubtyping1 A1 A2.
-     forwards*: IHsubtyping2 A1 A2.
-     unfold btmLikeSpec in *.
-     intros.
-     clear IHsubtyping1 IHsubtyping2.
-     unfold not. intros.
-     forwards*: H H1.
-     forwards*: H0 H1.
-     unfold not in *.
-     apply sub_and in H2.
-     destruct H2.
-     apply ord_sub_union in H5; auto.
-     destruct H5.
-     apply H3. apply s_anda; auto.
-     apply H4. apply s_anda; auto.
-   + forwards*: IHsubtyping A1 A2.
-     unfold btmLikeSpec in *.
-     intros.
-     unfold not in *. intros.
-     lets: H A H1.
-     apply sub_and in H2.
-     destruct H2.
-     apply sub_and in H4.
-     destruct H4.
-     apply H3.
-     apply s_anda; auto.
-   + forwards*: IHsubtyping A1 A2.
-     unfold btmLikeSpec in *. intros.
-     unfold not in *. intros.
-     eapply H; eauto.
-     apply sub_and in H2.
-     destruct H2.
-     apply sub_and in H3.
-     destruct H3.
-     apply s_anda; auto.
-  - forwards*: IHsubtyping1 A0 A3.
-    forwards*: IHsubtyping2 A0 A3.
-    unfold btmLikeSpec in *.
-    intros.
-    unfold not in *.
-    intros.
-    apply sub_and in H5.
-    destruct H5.
-    apply ord_sub_union in H5; auto.
-    destruct H5.
-    eapply H2; eauto.
-    eapply H3; eauto.
-  - forwards*: IHsubtyping A0 A3.
-    unfold btmLikeSpec in *.
-    unfold not in *.
-    intros.
-    eapply H1; eauto.
-    apply sub_and in H3.
-    destruct H3.
-    apply sub_and in H3. destruct H3.
-    apply s_anda; auto.
-  - forwards*: IHsubtyping A0 A3.
-    unfold btmLikeSpec in *.
-    unfold not in *.
-    intros.
-    eapply H1; eauto.
-    apply sub_and in H3. destruct H3.
-    eapply sub_and in H3. destruct H3.
-    apply s_anda; auto.
-Defined.
-
-Lemma sym_btm_like : forall A B, btmLikeSpec (t_and A B) -> btmLikeSpec (t_and B A).
-Proof.
-  intros.
-  unfold btmLikeSpec in *.
-  intros.
-  unfold not in *.
-  intros.
-  eapply H; eauto.
-  apply sub_and in H1.
-  destruct H1.
-  apply s_anda; auto.
-Defined.
-
-
-Lemma disj_btm_like_spec : forall A B, A *s B ->
-  forall C, C <: A -> C <: B -> btmLikeSpec C.
-Proof.
- intros.
- unfold DisjSpec in H.
- apply H; eauto.
-Defined.
-
-Lemma disj_sub_union : forall A B C, A *s C -> B *s C -> t_union A B *s C.
-Proof.
-  intros.
-  unfold DisjSpec in *. intros.
-  unfold btmLikeSpec in *. intros.
-  destruct H1.
-  unfold not. intros.
-  specialize (H A0).
-  eapply sub_transitivity in H3; eauto.
-  eapply sub_transitivity in H1; eauto.
-  lets: ord_sub_union A0 H2 A B H1.
-  destruct H5.
-  unfold not in *.
-  assert (A0 <: A /\ A0 <: C) by auto.
-  lets: H H6.
-  forwards*: H7 H2.
-  specialize (H0 A0).
-  assert (A0 <: B /\ A0 <: C) by auto.
-  lets: H0 H6.
-  unfold not in H7.
-  forwards*: H7 H2.
-Defined.
-
-Lemma disj_spec_union : forall A B C, t_union A B *s C -> A *s C /\ B *s C.
-Proof.
-  unfold DisjSpec; unfold btmLikeSpec; unfold not; intros.
-  split.
-  - intros. destruct H0.
-    specialize (H C0).
-    apply H with (A:=A0); auto.
-  - intros. destruct H0.
-    specialize (H C0).
-    apply H with (A:=A0); auto.
-Defined.
-
-Lemma disj_spec_union1 : forall A B C, A *s t_union B C -> A *s B /\ A *s C.
-Proof.
-  unfold DisjSpec; unfold btmLikeSpec; unfold not; intros.
-  split.
-  - intros. destruct H0.
-    specialize (H C0).
-    apply H with (A:=A0); auto.
-  - intros. destruct H0.
-    specialize (H C0).
-    apply H with (A:=A0); auto.
-Defined.
-
-
-Lemma ord_sub_disj_spec_false : forall A, Ord A -> 
-forall B C, B *s C -> A <: (t_and B C) -> False.
-Proof.
- intros.
- unfold DisjSpec in H0.
- unfold btmLikeSpec in H0. unfold not in H0.
- apply sub_and in H1. destruct H1.
- specialize (H0 (t_and B C)).
- forwards*: H0 H.
-Defined.
-
-Lemma BL_disj : forall A, bottomlike A -> forall B, A *a B.
-Proof.
-  intros A H1.
-  inductions H1; intros; eauto.
-Defined.
-
-Lemma Disj_sym_spec : forall A B, A *s B -> B *s A.
-Proof.
-  unfold DisjSpec. intros.
-  destruct H0.
-  apply* H.
-Defined.
-
-Lemma BL_soundness : forall A, bottomlike A -> btmLikeSpec A
-with Disj_soundness : forall A B, A *a B -> A *s B.
-Proof.
-(* BL_soundness Soundness Proof *)
-- clear BL_soundness. intros. inductions H; unfold btmLikeSpec in *; intros.
- + unfold not. intros.
-  inductions H; try solve [inversion H0].
- + specialize (IHbottomlike1 A0).
-  specialize (IHbottomlike2 A0).
-  forwards: IHbottomlike1. auto.
-  forwards: IHbottomlike2. auto.
-  clear IHbottomlike1 IHbottomlike2.
-  unfold not. intros.
-  dependent induction H4; auto.
-  inversion H1. inversion H1. inversion H1.
- + specialize (IHbottomlike A0).
-  forwards: IHbottomlike. auto.
-  unfold not in *. intros.
-  apply H1.
-  apply sub_and in H2. destruct H2. auto.
- + specialize (IHbottomlike A0).
-  forwards: IHbottomlike. auto.
-  unfold not in *. intros.
-  apply H1.
-  apply sub_and in H2. destruct H2. auto.
- + unfold not in *.
-  intros.
-  apply Disj_soundness in H.
-  lets: ord_sub_disj_spec_false A0 H0 A B H.
-  forwards: H2 H1. auto.
-
-(* Disj_soundness Soundness Proof *)
-- clear Disj_soundness. intros. dependent induction H; unfold DisjSpec; intros.
- + apply BL_soundness in H.
-   destruct H0.
-   unfold btmLikeSpec in *. unfold not in *. intros.
-   specialize (H A0 H2).
-   apply H.
-   apply sub_transitivity with (A := A0) (B := C) (C := A).
-   auto. auto.
- + apply BL_soundness in H.
-   destruct H0.
-   unfold btmLikeSpec in *. unfold not in *. intros.
-   specialize (H A0 H2).
-   apply H.
-   apply sub_transitivity with (A := A0) (B := C) (C := B).
-   auto. auto.
- + destruct H. induction C; try (dependent destruction H).
-  * inversion H0.
-  * apply btm_spec.
-  * inverts* H1.
-    forwards*: IHC1.
-    forwards*: IHC2.
-    apply* btm_like_spec_union_inv.
-  * inverts* H0.
-    forwards*: IHC1.
-    apply* btm_like_spec_and1_inv.
-    eapply sub_int_arrow; eauto.
-  * inverts* H0.
-    apply sym_btm_like.
-    eapply sub_int_arrow; eauto.
-    forwards*: IHC2.
-    apply* btm_like_spec_and2_inv.
-+ destruct H. induction C; try (dependent destruction H0).
-  * inversion H.
-  * apply btm_spec.
-  * inverts* H.
-    forwards*: IHC1.
-    forwards*: IHC2.
-    apply* btm_like_spec_union_inv.
-  * inverts* H.
-    forwards*: IHC1.
-    apply* btm_like_spec_and1_inv.
-    eapply sub_int_arrow; eauto.
-  * inverts* H.
-    apply sym_btm_like.
-    eapply sub_int_arrow; eauto.
-    forwards*: IHC2.
-    apply* btm_like_spec_and2_inv.
-    (* difficult case -- union with intersection *)
-+ destruct H1.
-  lets: disj_sub_union A B C IHdisjointness1 IHdisjointness2.
-  unfold DisjSpec in H3.
-  apply H3. split. auto. auto.
-    (* difficult case -- union with intersection *)
-+ destruct H1.
-  apply Disj_sym_spec in IHdisjointness1.
-  apply Disj_sym_spec in IHdisjointness2.
-  lets: disj_sub_union B C A IHdisjointness1 IHdisjointness2.
-  unfold DisjSpec in H3.
-  apply H3. split. auto. auto.
- + destruct H0.
-  unfold DisjSpec in IHdisjointness.
-  apply IHdisjointness.
-  split; auto.
-  apply sub_and in H0. destruct H0; auto.
- + destruct H0.
-  unfold DisjSpec in IHdisjointness.
-  apply IHdisjointness.
-  split; auto.
-  apply sub_and in H0.
-  destruct H0; auto.
- + destruct H0.
-  apply sub_and in H1.
-  destruct H1.
-  unfold DisjSpec in IHdisjointness.
-  apply IHdisjointness; auto.
- + destruct H0.
-  apply sub_and in H1.
-  destruct H1.
-  unfold DisjSpec in IHdisjointness.
-  apply IHdisjointness; auto.
-Qed.
-
-Lemma BL_disj_spec : forall A, btmLikeSpec A -> forall B, A *s B.
-  intros.
-  unfold btmLikeSpec in H.
-  unfold not in H.
-  unfold DisjSpec. intros.
-  unfold btmLikeSpec. intros.
-  unfold not. intros.
-  eapply H; eauto.
-  destruct H0.
-  eapply sub_transitivity; eauto.
-Defined.
-
-Lemma disj_btm_spec : forall A B, A *s B -> btmLikeSpec (t_and A B).
-Proof.
-  intros.
-  unfold DisjSpec in H.
-  apply H; eauto.
-Defined.
-
-Lemma Disj_sym : forall A B, A *a B -> B *a A.
-  induction 1; eauto.
-Defined.
-
-Lemma bl_union_inv : forall A B, bottomlike (t_union A B) -> 
-bottomlike A /\ bottomlike B.
-Proof.
-intros. inverts* H.
-Defined.
-
-Lemma disj_union_inv : forall A B C, A *a (t_union B C) ->
-  A *a B /\ A *a C.
-Proof.
-intros.
-inductions H; eauto.
-- apply bl_union_inv in H.
-  destruct H. split*.
-- specialize (IHdisjointness1 B C).
-  destruct IHdisjointness1; auto.
-  specialize (IHdisjointness2 B C).
-  destruct IHdisjointness2; auto.
-- specialize (IHdisjointness B C).
-  destruct IHdisjointness; auto.
-- specialize (IHdisjointness B C).
-  destruct IHdisjointness; auto.
-Defined.
-
-
-Lemma ord_sub_int_arrow_false : forall A B A1 A2, Ord A -> A <: B -> B <: t_int -> B <: t_arrow A1 A2 -> False.
-Proof.
-  intros.
-  lets: sub_int_arrow B B H1 A1 A2.
-  forwards*: H3.
-  unfold btmLikeSpec in H4.
-  unfold not in H4.
-  eapply H4; eauto.
-Defined.
-
-(***************************)
-(*
-
-Important lemma for completeness.
-
-\/ A B, botlike((A & B) & Int) -> botlike (A & Int) \/ botlike (B & Int)
-
-Below is the proof of this lemma.
-
-Difficult to prove.
-
-*)
-(***************************)
-
-Lemma btm_like_spec_int_and : forall A B, btmLikeSpec (t_and (t_and A B) t_int) -> 
-  btmLikeSpec (t_and A t_int) \/ btmLikeSpec (t_and B t_int).
-Proof.
-  intros.
-  unfold btmLikeSpec in *.
-  unfold not in *.
-  inductions A; eauto.
-  - right. intros.
-    apply sub_and in H1. destruct H1.
-    forwards*: H A H0.
-  - right. intros.
-    apply sub_and in H1. destruct H1.
-    forwards*: H A H0.
-  - left. intros.
-    apply sub_and in H1. destruct H1.
-    forwards*: ord_sub_bot_false A H0.
-  - clear IHA1 IHA2.
-    left. intros. apply sub_and in H1.
-    destruct H1.
-    lets: sub_int_arrow A A H2 H1.
-    unfold btmLikeSpec in H3. unfold not in H3.
-    lets: H3 A H0.
-    apply H4; eauto.
-  - specialize (IHA1 B).
-    destruct IHA1. intros. apply sub_and in H1. destruct H1.
-    apply sub_and in H1. destruct H1.
-    eapply H; eauto.
-    specialize (IHA2 B).
-    destruct IHA2. intros.
-    apply sub_and in H2. destruct H2.
-    apply sub_and in H2. destruct H2.
-    eapply H; eauto.
-    left. intros.
-    apply sub_and in H3. destruct H3.
-    lets: ord_sub_union A H2 A1 A2 H3.
-    destruct H5.
-    eapply H0; eauto.
-    eapply H1; eauto.
-    right. auto.
-    specialize (IHA2 B). destruct IHA2.
-    intros. apply sub_and in H2. destruct H2.
-    apply sub_and in H2. destruct H2.
-    eapply H; eauto.
-    right. auto. right. auto.
-  - specialize (IHA1 (t_and A2 B)). destruct IHA1.
-    specialize (IHA2 (t_and A1 B)). destruct IHA2.
-    intros. apply sub_and in H1. destruct H1.
-    apply sub_and in H1. destruct H1.
-    apply sub_and in H3. destruct H3.
-    eapply H; eauto.
-    intros. apply sub_and in H2. destruct H2.
-    apply sub_and in H2. destruct H2.
-    apply sub_and in H4. destruct H4.
-    eapply H0; eauto.
-    intros. apply sub_and in H2. destruct H2.
-    apply sub_and in H2. destruct H2.
-    apply sub_and in H4. destruct H4.
-    eapply H0; eauto.
-    specialize (IHA2 A1). destruct IHA2.
-    intros.
-    apply sub_and in H2. destruct H2.
-    apply sub_and in H2. destruct H2.
-    eapply H0; eauto.
-    left. intros.
-    apply sub_and in H3. destruct H3.
-    apply sub_and in H3. destruct H3.
-    eapply H0; eauto.
-    left. intros.
-    apply sub_and in H3. destruct H3.
-    apply sub_and in H3. destruct H3.
-    eapply H0; eauto.
-    specialize (IHA2 B). destruct IHA2.
-    intros.
-    apply sub_and in H2. destruct H2.
-    apply sub_and in H2. destruct H2.
-    eapply H0; eauto.
-    left. intros.
-    apply sub_and in H3. destruct H3.
-    apply sub_and in H3. destruct H3.
-    eapply H1; eauto.
-    right. auto.
-Defined.
-
-
-(***************************)
-(*
-
-Important lemma for completeness.
-
-\/ A B, botlike((A & B) & (A1 -> B1)) -> botlike (A & (A1 -> B1)) \/ botlike (B & (A1 -> B1))
-
-Below is the proof of this lemma.
-
-Difficult to prove.
-
-*)
-(***************************)
-
-Lemma ord_sub_arrow_and_B : forall A, Ord A -> forall B, A <: B -> 
-forall A1 A2, A <: (t_arrow A1 A2) -> exists A3 A4, A = (t_arrow A3 A4).
-Proof.
-  intros.
-  dependent induction H1; eauto; try solve [inversion H].
-Defined.
-
-Lemma btm_like_spec_arrow_and : forall A B A1 B1, btmLikeSpec (t_and (t_and A B) (t_arrow A1 B1)) -> 
-  btmLikeSpec (t_and A (t_arrow A1 B1)) \/ btmLikeSpec (t_and B (t_arrow A1 B1)).
-Proof.
-  intros.
-  unfold btmLikeSpec in *.
-  unfold not in *.
-  inductions A; eauto.
-    (* Top Case *)
-  - right. intros.
-    apply sub_and in H1. destruct H1.
-    forwards*: H A H0.
-    (* Int Case *)
-  - left. intros.
-    apply sub_and in H1. destruct H1.
-    lets: sub_int_arrow A A H1 A1 B1.
-    lets: H3 H2.
-    unfold btmLikeSpec in H4. unfold not in H4.
-    forwards*: H4 H0.
-    (* Bottom Case *)
-  - left. intros.
-    apply sub_and in H1. destruct H1.
-    forwards*: ord_sub_bot_false A H0.
-    (* Arrow Case *)
-  - right. intros.
-    apply sub_and in H1.
-    destruct H1.
-    lets: ord_sub_arrow_and_B A H0 B H1.
-    lets: H3 A0 B1 H2.
-    destruct H4 as [A3 [A4]].
-    clear H3.
-    subst.
-    specialize (H (t_arrow typ_top t_bot)).
-    forwards*: H.
-    apply* s_anda.
-    apply* s_anda.
-    assert ((t_arrow typ_top t_bot) <: (t_arrow A3 A4)) by eauto.
-    eapply sub_transitivity; eauto.
-    
-    (* Below is old and inefficient approach to prove this case *)
-    (* By induction on the subtyping relation of Ord type and arrow type *)
-
-    (*inductions H2; eauto; try solve [inversion H0];
-    clear IHsubtyping1 IHsubtyping2 IHA1 IHA2.
-    specialize (H (t_arrow typ_top t_bot)).
-    forwards*: H.
-    apply* s_anda.
-    apply* s_anda.
-    assert ((t_arrow typ_top t_bot) <: (t_arrow A4 A3)) by eauto.
-    eapply sub_transitivity; eauto.*)
-    (* union Case *)
-  - specialize (IHA1 B A0 B1).
-    destruct IHA1. intros. apply sub_and in H1. destruct H1.
-    apply sub_and in H1. destruct H1.
-    eapply H; eauto.
-    specialize (IHA2 B A0 B1).
-    destruct IHA2. intros.
-    apply sub_and in H2. destruct H2.
-    apply sub_and in H2. destruct H2.
-    eapply H; eauto.
-    left. intros.
-    apply sub_and in H3. destruct H3.
-    lets: ord_sub_union A H2 A1 A2 H3.
-    destruct H5.
-    eapply H0; eauto.
-    eapply H1; eauto.
-    right. auto.
-    specialize (IHA2 B A0 B1). destruct IHA2.
-    intros. apply sub_and in H2. destruct H2.
-    apply sub_and in H2. destruct H2.
-    eapply H; eauto.
-    right. auto. right. auto.
-    (* Intersection case *)
-  - specialize (IHA1 (t_and A2 B) A0 B1). destruct IHA1.
-    specialize (IHA2 (t_and A1 B) A0 B1). destruct IHA2.
-    intros. apply sub_and in H1. destruct H1.
-    apply sub_and in H1. destruct H1.
-    apply sub_and in H3. destruct H3.
-    eapply H; eauto.
-    intros. apply sub_and in H2. destruct H2.
-    apply sub_and in H2. destruct H2.
-    apply sub_and in H4. destruct H4.
-    eapply H0; eauto.
-    intros. apply sub_and in H2. destruct H2.
-    apply sub_and in H2. destruct H2.
-    apply sub_and in H4. destruct H4.
-    eapply H0; eauto.
-    specialize (IHA2 A1 A0 B1). destruct IHA2.
-    intros.
-    apply sub_and in H2. destruct H2.
-    apply sub_and in H2. destruct H2.
-    eapply H0; eauto.
-    left. intros.
-    apply sub_and in H3. destruct H3.
-    apply sub_and in H3. destruct H3.
-    eapply H0; eauto.
-    left. intros.
-    apply sub_and in H3. destruct H3.
-    apply sub_and in H3. destruct H3.
-    eapply H0; eauto.
-    specialize (IHA2 B A0 B1). destruct IHA2.
-    intros.
-    apply sub_and in H2. destruct H2.
-    apply sub_and in H2. destruct H2.
-    eapply H0; eauto.
-    left. intros.
-    apply sub_and in H3. destruct H3.
-    apply sub_and in H3. destruct H3.
-    eapply H1; eauto.
-    right. auto.
-Defined.
-
-Lemma disj_spec_int : forall A1 A2, (t_and A1 A2) *s t_int -> A1 *s t_int \/ A2 *s t_int.
-Proof.
-  intros.
-  unfold DisjSpec in *.
-  unfold btmLikeSpec in *.
-  unfold not in *.
-  specialize (H (t_and (t_and A1 A2) t_int)).
-  assert ((t_and (t_and A1 A2) t_int <: t_and A1 A2)) by auto.
-  assert (t_and (t_and A1 A2) t_int <: t_int) by auto.
-  assert ((t_and (t_and A1 A2) t_int <: t_and A1 A2) /\ (t_and (t_and A1 A2) t_int <: t_int)) by auto.
-  lets: H H2.
-  clear H H0 H1 H2.
-  inductions A1; eauto.
-  - inductions A2; eauto.
-    + right. intros.
-      destruct H.
-      assert (A <: t_bot).
-      eapply sub_transitivity; eauto.
-      lets: ord_sub_bot_false A H0 H4. auto.
-    + clear IHA2_1 IHA2_2.
-      right. intros. destruct H.
-      forwards*: ord_sub_int_arrow_false H1.
-    + clear IHA2_1 IHA2_2.
-      right. intros. destruct H.
-      lets H2': H2. 
-      inverts* H2; eauto.
-      lets: ord_sub_bot_false A H0 H1. auto.
-      assert (A <: t_int).
-      eapply sub_transitivity; eauto.
-      eapply sub_transitivity in H; eauto.
-      assert (A <: t_int).
-      eapply sub_transitivity; eauto.
-      eapply sub_transitivity in H; eauto.
-      assert (A <: t_int).
-      eapply sub_transitivity; eauto.
-      eapply sub_transitivity in H; eauto.
-    + clear IHA2_1 IHA2_2.
-      right. intros. destruct H.
-      lets H2': H2.
-      inverts* H2; eauto.
-      lets: ord_sub_bot_false A H0 H1. auto.
-      assert (A <: t_int).
-      eapply sub_transitivity; eauto.
-      eapply sub_transitivity in H; eauto.
-      assert (A <: t_int).
-      eapply sub_transitivity; eauto.
-      eapply sub_transitivity in H; eauto.
-      assert (A <: t_int).
-      eapply sub_transitivity; eauto.
-      eapply sub_transitivity in H; eauto.
-  - inductions A2; eauto.
-    + right. intros.
-      destruct H.
-      assert (A <: t_bot).
-      eapply sub_transitivity; eauto.
-      lets: ord_sub_bot_false A H0 H4. auto.
-    + right. intros.
-      destruct H.
-      lets: ord_sub_int_arrow_false A C A2_1 A2_2 H0.
-      lets: H4 H1 H2 H. auto.
-    + right. intros. destruct H.
-      lets H2': H2.
-      dependent destruction H2; eauto.
-      forwards*: ord_sub_bot_false A H0 H1.
-      assert (A <: t_int).
-      eapply sub_transitivity; eauto.
-      eapply sub_transitivity in H; eauto.
-      assert (A <: t_int).
-      eapply sub_transitivity; eauto.
-      eapply sub_transitivity in H; eauto.
-      assert (A <: t_int).
-      eapply sub_transitivity; eauto.
-      eapply sub_transitivity in H; eauto.
-    + right. intros. destruct H.
-      lets H2': H2.
-      dependent destruction H2; eauto.
-      forwards*: ord_sub_bot_false A H0 H1.
-      assert (A <: t_int).
-      eapply sub_transitivity; eauto.
-      eapply sub_transitivity in H; eauto.
-      assert (A <: t_int).
-      eapply sub_transitivity; eauto.
-      eapply sub_transitivity in H; eauto.
-      assert (A <: t_int).
-      eapply sub_transitivity; eauto.
-      eapply sub_transitivity in H; eauto.
-  - left. intros. destruct H.
-    assert (A <: t_bot ).
-    eapply sub_transitivity; eauto.
-    forwards*: ord_sub_bot_false A H0 H4.
-  - clear IHA1_1 IHA1_2.
-    left. intros.
-    destruct H.
-    lets: ord_sub_int_arrow_false A C A1_1 A1_2 H0.
-    lets: H4 H1 H2 H. auto.
-  - clear IHA1_1 IHA1_2. inductions A2; eauto.
-    + left. intros.
-      destruct H.
-      assert (A <: t_int).
-      eapply sub_transitivity; eauto.
-      eapply sub_transitivity in H; eauto.
-    + left. intros.
-      destruct H.
-      assert (A <: t_int).
-      eapply sub_transitivity; eauto.
-      eapply sub_transitivity in H; eauto.
-    + right. intros. destruct H.
-      assert (A <: t_bot).
-      eapply sub_transitivity; eauto.
-      forwards*: ord_sub_bot_false A H0 H4.
-    + clear IHA2_1 IHA2_2. right. intros.
-      destruct H.
-      lets: ord_sub_int_arrow_false A C A2_1 A2_2 H0.
-      lets: H4 H1 H2 H. auto.
-    + clear IHA2_1 IHA2_2.
-      apply btm_like_spec_int_and in H3.
-      destruct H3.
-      left. intros.
-      unfold btmLikeSpec in H.
-      unfold not in H.
-      destruct H0.
-      assert (A <: t_int).
-      eapply sub_transitivity; eauto.
-      eapply sub_transitivity in H0; eauto.
-      right. intros. destruct H0.
-      unfold btmLikeSpec in H.
-      unfold not in H.
-      assert (A <: t_int).
-      eapply sub_transitivity; eauto.
-      eapply sub_transitivity in H0; eauto.
-    + clear IHA2_1 IHA2_2.
-      apply btm_like_spec_int_and in H3.
-      destruct H3.
-      unfold btmLikeSpec in H.
-      unfold not in H.
-      left. intros. destruct H0.
-      assert (A <: t_int).
-      eapply sub_transitivity; eauto.
-      eapply sub_transitivity in H0; eauto.
-      unfold btmLikeSpec in H.
-      unfold not in H.
-      right. intros. destruct H0.
-      assert (A <: t_int).
-      eapply sub_transitivity; eauto.
-      eapply sub_transitivity in H0; eauto.
-  - clear IHA1_1 IHA1_2.
-    apply btm_like_spec_int_and in H3.
-    destruct H3.
-    unfold btmLikeSpec in H.
-    unfold not in H.
-    left. intros. destruct H0.
-    assert (A <: t_int).
-    eapply sub_transitivity; eauto.
-    eapply sub_transitivity in H0; eauto.
-    unfold btmLikeSpec in H.
-    unfold not in H.
-    right. intros. destruct H0.
-    assert (A <: t_int).
-    eapply sub_transitivity; eauto.
-    eapply sub_transitivity in H0; eauto.
-Defined.
-
-
-Lemma disj_spec_arrow : forall A1 A2 B1 B2, (t_and A1 A2) *s (t_arrow B1 B2) -> 
-A1 *s (t_arrow B1 B2) \/ A2 *s (t_arrow B1 B2).
-Proof.
-  intros.
-  unfold DisjSpec in *.
-  unfold btmLikeSpec in *.
-  unfold not in *.
-  specialize (H (t_and (t_and A1 A2) (t_arrow B1 B2))).
-  assert ((t_and (t_and A1 A2) (t_arrow B1 B2) <: t_and A1 A2)) by auto.
-  assert (t_and (t_and A1 A2) (t_arrow B1 B2) <: (t_arrow B1 B2)) by auto.
-  assert ((t_and (t_and A1 A2) (t_arrow B1 B2) <: t_and A1 A2) /\ (t_and (t_and A1 A2) (t_arrow B1 B2) <: (t_arrow B1 B2))) by auto.
-  lets: H H2.
-  clear H H0 H1 H2.
-  apply btm_like_spec_arrow_and in H3.
-  destruct H3.
- - unfold btmLikeSpec in H.
-   unfold not in H.
-   left. intros.
-   destruct H0.
-   assert (A <: A1). eapply sub_transitivity; eauto.
-   eapply sub_transitivity in H3; eauto.
- - unfold btmLikeSpec in H. unfold not in H.
-   right. intros.
-   destruct H0.
-   assert (A <: A2). eapply sub_transitivity; eauto.
-   eapply sub_transitivity in H3; eauto.
-Defined.
-
-Lemma disj_spec_int_extra : forall A1 A2, (t_and A1 A2) *s t_int -> A1 *s t_int \/ A2 *s t_int.
-Proof.
-  intros.
-  unfold DisjSpec in *.
-  unfold btmLikeSpec in *.
-  unfold not in *.
-  specialize (H (t_and (t_and A1 A2) t_int)).
-  assert ((t_and (t_and A1 A2) t_int <: t_and A1 A2)) by auto.
-  assert (t_and (t_and A1 A2) t_int <: t_int) by auto.
-  assert ((t_and (t_and A1 A2) t_int <: t_and A1 A2) /\ (t_and (t_and A1 A2) t_int <: t_int)) by auto.
-  lets: H H2.
-  clear H H0 H1 H2.
-  apply btm_like_spec_int_and in H3.
-  destruct H3.
-  - unfold btmLikeSpec in H.
-    unfold not in H.
-    left. intros.
-    destruct H0.
-    assert (A <: t_int). eapply sub_transitivity; eauto.
-    eapply sub_transitivity in H0; eauto.
-  - unfold btmLikeSpec in H.
-    unfold not in H.
-    right. intros.
-    destruct H0.
-    assert (A <: t_int). eapply sub_transitivity; eauto.
-    eapply sub_transitivity in H0; eauto.
-Defined.
-
-Lemma top_btmlike : forall A, btmLikeSpec (t_and typ_top A) -> btmLikeSpec A.
-Proof.
-  intros.
-  unfold btmLikeSpec in *.
-  unfold not in *.
-  intros.
-  forwards*: H H0.
-Defined.
-
-Lemma top_disj : forall A, typ_top *s A -> btmLikeSpec A.
-Proof.
-  intros.
-  apply disj_btm_spec in H.
-  apply top_btmlike in H.
-  apply H.
-Defined.
-
-Lemma disj_spec_and_top : forall A1 A2, (t_and A1 A2) *s typ_top -> A1 *s A2.
-Proof.
-  intros.
-  unfold DisjSpec in *.
-  intros.
-  destruct H0.
-  eapply H; eauto.
-Defined.
-
-
-Lemma btm_like_spec_union_inter : forall A1 A2 B1 B2, btmLikeSpec (t_and (t_and A1 A2) (t_union B1 B2)) ->
-btmLikeSpec (t_and (t_and A1 A2) B1) /\ btmLikeSpec (t_and (t_and A1 A2) B2).
-Proof.
-  intros.
-  unfold btmLikeSpec in *.
-  unfold not in *.
-  split.
-  - intros.
-    apply sub_and in H1. destruct H1.
-    eapply H; eauto.
-  - intros.
-    apply sub_and in H1. destruct H1.
-    eapply H; eauto.
-Defined.
-
-
-Lemma disj_spec_union_inter_or : forall A1 A2 B1 B2, t_and A1 A2 *s t_union B1 B2 ->
-t_and A1 A2 *s B1 /\ t_and A1 A2 *s B2.
-Proof.
-  intros.
-  unfold DisjSpec in *.
-  eapply btm_like_spec_union_inter in H; eauto.
-  destruct H. split.
- - intros. destruct H1.
-  unfold btmLikeSpec in *. unfold not in *.
-  intros.
-  assert (A <: B1). eapply sub_transitivity; eauto.
-  eapply sub_transitivity in H1; eauto.
- - intros. destruct H1.
-   unfold btmLikeSpec in *. unfold not in *.
-   intros.
-   assert (A <: B2). eapply sub_transitivity; eauto.
-   eapply sub_transitivity in H1; eauto.
-Defined.
-
-(* 
-
-Following two lemmas seem true but can't figure our how to prove
-
-test61 depends upon test6
-
-Did not find any counter example and can't prove the lemma
-
-God help this poor PhD student! Please!
-
-*)
-
-Lemma test62 : forall A B C, Ord A -> not (A <: B) -> not (A <: (t_and B C)).
-Proof.
-  intros.
-  unfold not in *.
-  intros.
-  apply sub_and in H1. destruct H1.
-  apply H0; auto.
-Qed.
-
-Lemma test6 : forall A1 A2 B, btmLikeSpec (t_and (t_and A1 A2) B) ->
-btmLikeSpec (t_and A1 B) \/ btmLikeSpec (t_and A2 B) \/ btmLikeSpec (t_and A1 A2).
-Proof.
-  intros.
-  unfold btmLikeSpec in *.
-  unfold not in *.
-  left.
-  intros.
-  apply sub_and in H1. destruct H1.
-Admitted.
-
-Lemma test61 : forall B A1 A2, (t_and A1 A2) *s B ->
-A1 *s B \/ A2 *s B \/ A1 *s A2.
-Proof.
-  intros.
-  assert (btmLikeSpec (t_and(t_and A1 A2) B)). eauto.
-  apply test6 in H0.
-  destruct H0.
-  left.
-  unfold DisjSpec.
-  intros.
-  unfold btmLikeSpec in *.
-  unfold not in *.
-  intros.
-  destruct H1.
-  assert (A <: B). eapply sub_transitivity; eauto.
-  eapply sub_transitivity in H1; eauto.
-  destruct H0.
-  right. left.
-  unfold DisjSpec. intros.
-  unfold btmLikeSpec in *. unfold not in *. intros.
-  destruct H1.
-  assert (A <: B). eapply sub_transitivity; eauto.
-  eapply sub_transitivity in H1; eauto.
-  right. right.
-  unfold DisjSpec. intros.
-  unfold btmLikeSpec in *. unfold not in *. intros.
-  destruct H1.
-  assert (A <: A2). eapply sub_transitivity; eauto.
-  eapply sub_transitivity in H1; eauto.
-Qed.
-
-Lemma disj_spec_or_top : forall A1 A2, (t_union A1 A2) *s typ_top -> A1 *s A2.
-Proof.
-  intros.
-  unfold DisjSpec in *. intros.
-  destruct H0.
-  eapply H; auto.
-Defined.
-
-Lemma disj_spec_or_top1 : forall A1 A2, btmLikeSpec(t_and (t_union A1 A2) typ_top) -> btmLikeSpec (t_union A1 A2).
-Proof.
-  intros.
-  unfold btmLikeSpec in *.
-  unfold not in *.
-  intros.
-  forwards*: H1.
-Defined.
-
-Lemma btm_like_disj_algo_top : forall A, bottomlike (t_and typ_top A) ->
-typ_top *a A.
-Proof.
-  intros.
-  inverts* H.
-Defined.
-
-Lemma btm_like_disj : forall A, bottomlike A -> forall B, A *a B.
-Proof.
-  induction 1; auto.
-Defined.
-
-Lemma btm_like_and_disjoint : forall A B, bottomlike (t_and A B) -> A *a B.
-Proof.
-  intros. inductions H.
-  apply ad_btml. auto.
-  apply ad_btmr. auto.
-  apply H.
-Defined.
-
-Lemma disjoint_implies_btm_like : forall A B, A *a B -> bottomlike (t_and A B).
-Proof.
-  intros. apply bl_andsub. auto.
-Defined.
-
-Lemma btm_like_and_disjoint1 : forall A B, bottomlike (t_and A B) -> 
-bottomlike A \/ bottomlike B \/ A *a B.
-Proof.
-  intros. inductions H.
-  left. auto.
-  right. left. auto.
-  right. right. apply H.
-Defined.
-
-Lemma disj_spec_arrow_false : forall A1 A2 B1 B2, t_arrow A1 A2 *s t_arrow B1 B2 -> False.
-Proof.
-  unfold DisjSpec; unfold btmLikeSpec; unfold not; intros.
-  specialize (H (t_arrow typ_top t_bot)).
-  forwards: H; auto.
-Defined.
-
-Fixpoint size_of_type (A : typ) : nat :=
-  match A with 
-  | t_bot         => 1
-  | t_int         => 1
-  | typ_top       => 1
-  | t_arrow A1 B1 => 1 + (size_of_type A1) + (size_of_type B1)
-  | t_union A1 B1 => 1 + (size_of_type A1) + (size_of_type B1)
-  | t_and A1 B1   => 1 + (size_of_type A1) + (size_of_type B1)
-  end.
-
-Require Import Omega.
-
-Lemma BL_completeness : forall n A, size_of_type A < n -> btmLikeSpec A -> bottomlike A
-with Disj_completeness : forall n A B, (size_of_type A) + (size_of_type B) < n ->   A *s B -> A *a B.
-Proof.
-  (* Bottom Like completeness proof *)
-- clear BL_completeness. induction n.
-  intros. induction A; try solve [simpl in H; inversion H].
-
-induction A; unfold btmLikeSpec; intro.
- + unfold not.
-   intros.
-   specialize (H0 typ_top).
-   forwards: H0; auto.
-   false.
- + unfold not. intros.
-   specialize (H0 t_int).
-   forwards: H0; auto.
-   false.
- + intros. apply bl_bot.
- + unfold not. intros.
-   specialize (H0 (t_arrow A1 A2)).
-   forwards: H0; auto.
-   false.
- + unfold not. intros. apply bl_or.
-  * apply IHA1. simpl in H. omega.
-  unfold btmLikeSpec.
-  intros.
-  unfold not in *. intros.
-  specialize (H0 A).
-  assert (A <: (t_union A1 A2)) by auto.
-  apply H0. auto. auto.
-  * apply IHA2. simpl in H. omega.
-  unfold btmLikeSpec.
-  intros.
-  unfold not in *. intros.
-  specialize (H0 A).
-  assert (A <: (t_union A1 A2)) by auto.
-  apply H0. auto. auto.
- + clear IHA1. clear IHA2. intros.
-  apply bl_andsub.
-  assert (btmLikeSpec (t_and A1 A2)) by auto.
-  lets: btm_like_spec_and A1 A2 H1.
-  specialize (Disj_completeness n A1 A2).
-  apply Disj_completeness in H2. apply H2.
-  simpl in H. omega.
-
-  (* Dijointness completeness proof *)
-- clear Disj_completeness.  
- induction n. intros.
- induction A; try solve [simpl in H; inversion H].
- induction A; intros.
-  (* Top Case *)
- + apply top_disj in H0.
-   specialize (BL_completeness n B).
-   apply ad_btmr.
-   apply BL_completeness.
-   simpl in H. omega.
-   apply H0. 
-   (* Int Case *)
- + induction B.
-  * specialize (H0 t_int).
-    assert (t_int <: t_int /\ t_int <: typ_top) by auto.
-    lets: H0 H1.
-    unfold btmLikeSpec in H2. unfold not in H2.
-    specialize (H2 t_int).
-    assert (Ord t_int) by auto.
-    assert (t_int <: t_int) by auto.
-    lets: H2 H3 H4. false.
-  * specialize (H0 t_int).
-    assert (t_int <: t_int /\ t_int <: t_int) by auto.
-    lets: H0 H1.
-    unfold btmLikeSpec in H2. unfold not in H2.
-    specialize (H2 t_int).
-    assert (Ord t_int) by auto.
-    assert (t_int <: t_int) by auto.
-    lets: H2 H3 H4. false.
-  * apply ad_btmr. apply bl_bot.
-  * apply ad_intl.
-  * apply disj_spec_union1 in H0. destruct H0.
-    apply ad_orr.
-    apply IHB1. simpl. simpl in H. omega.
-    apply H0.
-    apply IHB2.
-    simpl in H. simpl. omega.
-    apply H1.
-  * (* Intersection and Int case - requires hard helping lemma *)
-    apply Disj_sym_spec in H0.
-    apply disj_spec_int_extra in H0. destruct H0.
-    apply ad_andr1. apply IHB1.
-    simpl in H. simpl. omega. apply Disj_sym_spec. apply H0.
-    apply ad_andr2. apply IHB2. 
-    simpl in H. simpl. omega. apply Disj_sym_spec. apply H0.
-   (* Bottom Case *)
- + apply ad_btml. apply bl_bot.
-    (* Arrow Case *)
- + clear IHA1 IHA2.
-   induction B.
-  * specialize (H0 (t_arrow A1 A2)).
-    assert (t_arrow A1 A2 <: t_arrow A1 A2 /\ t_arrow A1 A2 <: typ_top) by auto.
-    lets: H0 H1.
-    unfold btmLikeSpec in H2. unfold not in H2.
-    specialize (H2 (t_arrow A1 A2)).
-    assert (Ord (t_arrow A1 A2)) by auto.
-    assert ( (t_arrow A1 A2) <: (t_arrow A1 A2)) by auto.
-    lets: H2 H3 H4. false.
-  * apply ad_intr.
-  * apply ad_btmr. apply bl_bot.
-  * apply disj_spec_arrow_false in H0. false.
-  * apply disj_spec_union1 in H0. destruct H0.
-    apply ad_orr.
-    apply IHB1. simpl in H. simpl. omega. apply H0.
-    apply IHB2. simpl in H. simpl. omega. apply H1.
-  * apply Disj_sym_spec in H0. apply disj_spec_arrow in H0. destruct H0.
-    apply ad_andr1. apply IHB1.
-    simpl in H. simpl. omega. apply Disj_sym_spec. apply H0.
-    apply ad_andr2. apply IHB2.
-    simpl in H. simpl. omega. apply Disj_sym_spec. apply H0.
-    (* Union Case *)
- + apply disj_spec_union in H0. destruct H0.
-   apply ad_orl.
-   apply IHA1.
-   simpl in H. omega. apply H0.
-   apply IHA2.
-   simpl in H. omega. apply H1.
-  (* Intersection Case *)
- + clear IHA1 IHA2.
-   apply test61 in H0.
-   destruct H0.
-   apply ad_andl1.
-   apply IHn. simpl in H. omega.
-   apply H0.
-   destruct H0.
-   apply ad_andl2.
-   apply IHn. simpl in H. omega.
-   apply H0.
-   apply ad_btml.
-   apply disjoint_implies_btm_like.
-   apply IHn. simpl in H. omega.
-   apply H0.
-Qed.
